Fixed lrGrammar theorems.

slr-parsing/lrGrammarDefScript.sml
@@ -5,148 +5,159 @@ relationTheory markerTheory boolSimps optionTheory rich_listTheory
 
 open symbolDefTheory grammarDefTheory boolLemmasTheory listLemmasTheory
 setLemmasTheory whileLemmasTheory parseTreeTheory followSetDefTheory
-yaccDefTheory parseProp1DefTheory parseProp2DefTheory
+yaccDefTheory parseProp1DefTheory parseProp2DefTheory uselessSymbolsTheory
 
-val _ = new_theory "lrGrammarDef"
+val _ = new_theory "lrGrammarDef";
+val _ = diminish_srw_ss ["list EQ"];
 
 val handleg = Define 
 `handleg g sf rhs (pfx,lhs,sfx) = 
-?sf'.RTC (rderives g) [NTS (startSym g)] sf' /\
-(sf'=pfx++[NTS lhs]++sfx) /\ (MEM (rule lhs rhs) (rules g)) /\
-(sf = pfx++rhs++sfx) /\ EVERY isTmnlSym sfx`
+∃sf'.RTC (rderives g) [NTS (startSym g)] sf' ∧
+(sf'=pfx++[NTS lhs]++sfx) ∧ (MEM (rule lhs rhs) (rules g)) ∧
+(sf = pfx++rhs++sfx) ∧ EVERY isTmnlSym sfx`;
 
 
 val viablePfx = Define 
-`viablePfx g (N,h) sf p = ?pfx sfx.handleg g sf h (pfx,N,sfx) /\
-IS_PREFIX (pfx++h) p`
+`viablePfx g (N,h) sf p = ∃pfx sfx.handleg g sf h (pfx,N,sfx) ∧
+IS_PREFIX (pfx++h) p`;
 
 
 val validItem = Define 
 `validItem g vp (item l (r1,r2)) = 
-   ?pfx sfx.
-     RTC (rderives g) [NTS (startSym g)] (pfx++[NTS l]++sfx) /\
-     rderives g (pfx++[NTS l]++sfx) (pfx++r1++r2++sfx) /\
-     MEM (rule l (r1 ++ r2)) (rules g) /\
-     (pfx++r1=vp)`
-
-
+   ∃pfx sfx.
+     RTC (rderives g) [NTS (startSym g)] (pfx++[NTS l]++sfx) ∧
+     rderives g (pfx++[NTS l]++sfx) (pfx++r1++r2++sfx) ∧
+     MEM (rule l (r1 ++ r2)) (rules g) ∧
+     (pfx++r1=vp)`;
 
 val itemlist_def = Define`
-  itemlist (stl : ((symbol # item list)  list)) = SND ((HD stl))`
+ itemlist (stl : ((('nts,'ts)symbol # ('nts,'ts)item list)  list)) 
+ = SND ((HD stl))`;
 
-val completeItem = Define `(completeItem (item l (r1, [])) = T) /\
-(completeItem (item l (r1, r2)) = F)`
+val completeItem = Define `(completeItem (item l (r1, [])) = T) ∧
+(completeItem (item l (r1, r2)) = F)`;
 
 
 val shiftReduce = store_thm ("shiftReduce",
-``(slrmac ag = SOME m) ==> validItl ag itl 
-==> (getState m itl sym = REDUCE (rule l r)) ==>
-(trans ag (initItems ag (rules ag), vp)  = SOME itl) ==>
-!e.MEM e itl ==> 
-(e=item l (r,[])) \/ ~(?l' r2 r1.e = item l' (r1,sym::r2))``,
+``(slrmac ag = SOME m) ⇒ validItl ag itl 
+⇒ (getState m itl sym = REDUCE (rule l r)) ⇒
+(trans ag (initItems ag (rules ag), vp)  = SOME itl) ⇒ isTmnlSym sym ⇒
+∀e.MEM e itl ⇒ 
+(e=item l (r,[])) ∨ ~(∃l' r2 r1.e = item l' (r1,sym::r2))``,
+
 SRW_TAC [] [] THEN
 `m = (sgoto ag, reduce ag)` by METIS_TAC [sgoto_exp] THEN
 SRW_TAC [] [] THEN
-`MEM (item l (r,[])) itl` by METIS_TAC [getState_mem_itl, sgoto_exp, validStates_def] THEN
+`MEM (item l (r,[])) itl` by METIS_TAC [getState_mem_itl, sgoto_exp, 
+					validStates_def] THEN
 Cases_on `e` THEN Cases_on `p` THEN Cases_on `r'` THEN
 FULL_SIMP_TAC (srw_ss()) [slrmac_def, LET_THM] THEN
-Cases_on `q=r` THEN FULL_SIMP_TAC (srw_ss()) [] THEN
-SRW_TAC [] [] THEN
-Cases_on `h=sym` THEN FULL_SIMP_TAC (srw_ss()) [] THEN
-`MEM (item s (q++[sym],t)) (sgoto ag itl sym)` by METIS_TAC [sgoto_mem] THEN
 FULL_SIMP_TAC (srw_ss()) [getState_def, LET_THM] THEN
-`?h t.(sgoto ag itl sym) = h::t` by METIS_TAC [list_mem1, list_mem2] THEN
-FULL_SIMP_TAC (srw_ss()) [] THEN
-Cases_on `reduce ag itl (sym2Str sym)` THEN FULL_SIMP_TAC (srw_ss()) [] THEN
-Cases_on `itemEqRuleList (h'::t') (h''::t'')` THEN FULL_SIMP_TAC (srw_ss()) [] THEN
-FULL_SIMP_TAC (srw_ss() ++ DNF_ss) [option_case_rwt, list_case_rwt, pairTheory.FORALL_PROD] THEN
-`?h t.reduce ag itl (sym2Str sym) = h::t` by METIS_TAC [list_mem1, list_mem2, NOT_CONS_NIL, APPEND] THEN
-FULL_SIMP_TAC (srw_ss() ++ boolSimps.COND_elim_ss) [] THEN
-FIRST_X_ASSUM (Q.SPECL_THEN [`vp`,`itl`, `h`] MP_TAC) THEN
-Cases_on `t''` THEN SRW_TAC [][])
+Cases_on `sgoto ag itl sym` THEN
+Cases_on `reduce ag itl (ts2str sym)` THEN
+FULL_SIMP_TAC (srw_ss()) [] THEN1
+
+(Cases_on `LENGTH t' = 0` THEN FULL_SIMP_TAC (srw_ss()) [] THEN
+ SRW_TAC [][] THEN
+ SPOSE_NOT_THEN ASSUME_TAC THEN SRW_TAC [][] THEN
+ `MEM (item n (q++[h],t)) (sgoto ag itl h)` by METIS_TAC [sgoto_mem] THEN
+ FIRST_X_ASSUM (Q.SPECL_THEN [`vp`,`itl`,`h`] MP_TAC) THEN SRW_TAC [][] THEN
+ Cases_on `t'` THEN FULL_SIMP_TAC (srw_ss()) [] THEN
+ METIS_TAC [MEM, rgr_r9eq]) THEN
+
+Cases_on `itemEqRuleList (h'::t') (h''::t'')` THEN FULL_SIMP_TAC (srw_ss()) [] THEN 
+SRW_TAC [][] THEN
+ SPOSE_NOT_THEN ASSUME_TAC THEN SRW_TAC [][] THEN
+ FIRST_X_ASSUM (Q.SPECL_THEN [`vp`,`itl`,`h`] MP_TAC) THEN SRW_TAC [][] THEN
+ Cases_on `t''` THEN FULL_SIMP_TAC (srw_ss()) []);
 
 
-val followSetEq = mk_thm ([], ``!g sym.s IN (followSetML g sym) = s IN (followSet g sym)``)
+val followSetEq = 
+    mk_thm ([], ``∀g sym.s IN (followSetML g sym) = s IN (followSet g sym)``);
 
-val _ = save_thm ("followSetEq", followSetEq)
+val _ = save_thm ("followSetEq", followSetEq);
 
 val reduce_not_mem = store_thm ("reduce_not_mem",
-``isTmnlSym sym ==> (reduce ag itl (sym2Str sym) = []) ==> 
-(!e.MEM e itl ==> (~?N r.(e=(item N (r,[]))) /\ (sym IN (followSet ag (NTS N)))))``,
+``isTmnlSym sym ⇒ (reduce ag itl (ts2str sym) = []) ⇒ 
+(∀e.MEM e itl ⇒ (~∃N r.(e=(item N (r,[]))) ∧ (sym IN (followSet ag (NTS N)))))``,
+
 Cases_on `itl` THEN SRW_TAC [] [] THENL[
-`(reduce ag [e] (sym2Str sym) ++ (reduce ag t (sym2Str sym)) = [])` by METIS_TAC [reduce_append, APPEND] THEN
+`(reduce ag [e] (ts2str sym) ++ (reduce ag t (ts2str sym)) = [])` 
+					by METIS_TAC [reduce_append, APPEND] THEN
 FULL_SIMP_TAC (srw_ss()) [] THEN
 Cases_on `e` THEN  
 Cases_on `p` THEN 
-Cases_on `item s (q,r') = item N (r,[])` THEN FULL_SIMP_TAC (srw_ss()) [] THEN
+Cases_on `item n (q,r') = item N (r,[])` THEN FULL_SIMP_TAC (srw_ss()) [] THEN
 FULL_SIMP_TAC (srw_ss()) [reduce_def] THEN
-Cases_on `sym` THEN FULL_SIMP_TAC (srw_ss()) [sym2Str_def, isTmnlSym_def] THEN
-Cases_on `TS s' IN followSetML ag (NTS N)` THEN FULL_SIMP_TAC (srw_ss()) [] THEN
-METIS_TAC [followSetEq],
+Cases_on `sym` THEN FULL_SIMP_TAC (srw_ss()) [ts2str_def, isTmnlSym_def] THEN
+Cases_on `TS t' IN followSet ag (NTS N)` THEN FULL_SIMP_TAC (srw_ss()) [],
 
 FULL_SIMP_TAC (srw_ss()) [rgr_r9eq, reduce_append] THEN
 SRW_TAC [] [] THEN
-`(reduce ag [h] (sym2Str sym) ++ reduce ag r1 (sym2Str sym) ++
-reduce ag [e] (sym2Str sym) ++ (reduce ag r2 (sym2Str sym)) = [])` by METIS_TAC [reduce_append, APPEND] THEN
-`reduce ag [e] (sym2Str sym) = []` by FULL_SIMP_TAC (srw_ss()) [] THEN
+`(reduce ag [h] (ts2str sym) ++ reduce ag r1 (ts2str sym) ++
+reduce ag [e] (ts2str sym) ++ (reduce ag r2 (ts2str sym)) = [])` by METIS_TAC [reduce_append, APPEND] THEN
+`reduce ag [e] (ts2str sym) = []` by FULL_SIMP_TAC (srw_ss()) [] THEN
 Cases_on `e` THEN  
 Cases_on `p` THEN 
-Cases_on `item s (q,r') = item N (r,[])` THEN FULL_SIMP_TAC (srw_ss()) [] THEN
+Cases_on `item n (q,r') = item N (r,[])` THEN FULL_SIMP_TAC (srw_ss()) [] THEN
 FULL_SIMP_TAC (srw_ss()) [reduce_def] THEN
-Cases_on `sym` THEN FULL_SIMP_TAC (srw_ss()) [sym2Str_def, isTmnlSym_def] THEN
-Cases_on `TS s' IN followSetML ag (NTS N)` THEN FULL_SIMP_TAC (srw_ss()) [] THEN
-METIS_TAC [followSetEq]])
-
-
+Cases_on `sym` THEN FULL_SIMP_TAC (srw_ss()) [ts2str_def, isTmnlSym_def] THEN
+Cases_on `TS t IN followSet ag (NTS N)` THEN FULL_SIMP_TAC (srw_ss()) []]);
 
 val shiftReduceGoto = store_thm ("shiftReduceGoto",
-``(slrmac ag = SOME m) ==> isTmnlSym sym ==> validItl ag itl ==> (getState m itl sym = GOTO s') ==>
-~?N r.MEM (item N (r,[])) itl /\ (sym IN (followSet ag (NTS N)))``,
+``(slrmac ag = SOME m) ⇒ isTmnlSym sym ⇒ validItl ag itl ⇒
+				 (getState m itl sym = GOTO s') ⇒
+~∃N r.MEM (item N (r,[])) itl ∧ (sym IN (followSet ag (NTS N)))``,
+
 SRW_TAC [] [] THEN
 `m = (sgoto ag, reduce ag)` by METIS_TAC [sgoto_exp] THEN
 SRW_TAC [] [] THEN
 FULL_SIMP_TAC (srw_ss()) [slrmac_def, LET_THM] THEN
-Cases_on `?pfx itl' sym'.
-               (trans ag (initItems ag (rules ag),pfx) = SOME itl') /\
+Cases_on `∃pfx itl' sym'. isTmnlSym sym' ∧
+               (trans ag (initItems ag (rules ag),pfx) = SOME itl') ∧
                case sgoto ag itl' sym' of
                   [] ->
-                    (case reduce ag itl' (sym2Str sym') of
+                    (case reduce ag itl' (ts2str sym') of
                         [] -> F
                      || [v12] -> F
                      || v12::v16::v17 -> T)
                || v8::v9 ->
-                    case reduce ag itl' (sym2Str sym') of
+                    case reduce ag itl' (ts2str sym') of
                        [] -> F
                     || [v20] -> T
                     || v20::v26::v27 -> T` THEN 
 FULL_SIMP_TAC (srw_ss()) [] THEN
-`SOME (sgoto ag,reduce ag)=SOME (sgoto ag,reduce ag)` by METIS_TAC [NOT_SOME_NONE] THEN
+
+`SOME (sgoto ag,reduce ag)=SOME (sgoto ag,reduce ag)` by 
+				 METIS_TAC [NOT_SOME_NONE] THEN
 FULL_SIMP_TAC (srw_ss()) [] THEN
 SRW_TAC [][] THEN
 FULL_SIMP_TAC (srw_ss()) [getState_def, LET_THM] THEN
-Cases_on `sgoto ag itl sym` THEN
-Cases_on `reduce ag itl (sym2Str sym)` THEN FULL_SIMP_TAC (srw_ss()) [] THENL[
+(Cases_on `sgoto ag itl sym` THEN
+Cases_on `reduce ag itl (ts2str sym)` THEN FULL_SIMP_TAC (srw_ss()) [] THENL[
 Cases_on `LENGTH t = 0` THEN FULL_SIMP_TAC (srw_ss()) [],
 METIS_TAC [reduce_not_mem],
-Cases_on `itemEqRuleList (h::t) (h'::t')` THEN FULL_SIMP_TAC (srw_ss()) []])
+Cases_on `itemEqRuleList (h::t) (h'::t')` THEN FULL_SIMP_TAC (srw_ss()) []]));
 
 
 
 val auggr_neqStartSym = store_thm ("auggr_neqStartSym", 
-``(auggr g st eof = SOME ag) ==> !n.MEM (rule n []) (rules ag) ==> ~(n=st)``,
+``(auggr g st eof = SOME ag) ⇒ ∀n.MEM (rule n []) (rules ag) ⇒ ~(n=st)``,
 SRW_TAC [] [auggr_def] THEN
 SRW_TAC [] [rules_def] THEN
-METIS_TAC [slemma1_4, nonTerminalsEq])
+METIS_TAC [slemma1_4, nonTerminalsEq]);
 
 
 val stackSyms_stl = store_thm ("stackSyms_stl", 
-``(doReduce m (e::t,stl,(s, itl)::csl) r = SOME (sl',stl',csl')) ==>
-(getState m itl e = REDUCE r) ==>
+``(doReduce m (e::t,stl,(s, itl)::csl) r = SOME (sl',stl',csl')) ⇒
+(getState m itl e = REDUCE r) ⇒
 (stackSyms stl' = stackSyms (pop stl (LENGTH (ruleRhs r))) ++  [NTS (ruleLhs r)])``,
+
 SRW_TAC [] [] THEN
 FULL_SIMP_TAC (srw_ss()) [doReduce_def, LET_THM] THEN
 SRW_TAC [] [] THEN
-FULL_SIMP_TAC (srw_ss() ++ DNF_ss) [option_case_rwt, list_case_rwt, pairTheory.FORALL_PROD] THEN
+FULL_SIMP_TAC (srw_ss() ++ DNF_ss) [option_case_rwt, list_case_rwt, 
+				    pairTheory.FORALL_PROD] THEN
 Cases_on `isNonTmnlSym e` THEN Cases_on `addRule stl r` THEN
 Cases_on `FST m (SND (HD (pop ((s,itl)::csl) (LENGTH (ruleRhs r)))))
                (NTS (ruleLhs r)) =
@@ -155,48 +166,50 @@ FULL_SIMP_TAC (srw_ss()) [] THEN
 Cases_on `pop ((s, itl)::csl) (LENGTH (ruleRhs r)) = []` THEN
 Cases_on `r` THEN
 FULL_SIMP_TAC (srw_ss()) [ruleLhs_def] THEN
-`stl'=((NTS s',
-            FST m (SND (HD (pop ((s,itl)::csl) (LENGTH l)))) (NTS s')),x)::
+`stl'=((NTS n,
+            FST m (SND (HD (pop ((s,itl)::csl) (LENGTH l)))) (NTS n)),x)::
               pop stl (LENGTH l)` by METIS_TAC [] THEN
 ONCE_ASM_REWRITE_TAC [] THEN
-SRW_TAC [] [stackSyms_def, ruleRhs_def])
+SRW_TAC [] [stackSyms_def, ruleRhs_def]);
 
 
-val validStlItems = Define `(validStlItems stl [] = T) /\
-(validStlItems stl (e::t) =  (isSuffix (itemFstRhs e) (stackSyms stl)) /\ validStlItems stl t)`
+val validStlItems = Define `(validStlItems stl [] = T) ∧
+(validStlItems stl (e::t) =  
+(isSuffix (itemFstRhs e) (stackSyms stl)) ∧ validStlItems stl t)`;
 
 val validStlItemsStack = Define 
-`(validStlItemsStack [] [e] = validStlItems ([]:((symbol # state) # ptree) list) (SND e)) /\
+`(validStlItemsStack [] [e] = 
+  validStlItems ([]:((('nts,'ts)symbol # ('nts,'ts)state) # ('nts,'ts)ptree) list) (SND e)) ∧
 (validStlItemsStack (h::stl) (e::csl) =  
- validStlItems (h::stl) (SND e) /\ validStlItemsStack stl csl) /\
-(validStlItemsStack _ _ = F)`
+ validStlItems (h::stl) (SND e) ∧ validStlItemsStack stl csl) ∧
+(validStlItemsStack _ _ = F)`;
 
-val validItemStack = Define `(validItemStack g [] = T) /\
+val validItemStack = Define `(validItemStack g [] = T) ∧
 (validItemStack g (e::rst) =  
-                       EVERY (validItem g (stackSyms (e::rst))) (SND (FST e)) /\ 
-                       validItemStack g rst )`
+                       EVERY (validItem g (stackSyms (e::rst))) (SND (FST e)) ∧ 
+                       validItemStack g rst )`;
 
 
 val validStlItems_append = store_thm ("validStlItems_append", 
-``!l1 l2.validStlItems stl (l1++l2) = validStlItems stl l1 /\ validStlItems stl l2``,
+``∀l1 l2.validStlItems stl (l1++l2) = validStlItems stl l1 ∧ validStlItems stl l2``,
 Induct_on `l1` THEN Induct_on `l2` THEN SRW_TAC [] [] THENL[
 METIS_TAC [APPEND, validStlItems],
 METIS_TAC [APPEND, validStlItems],
-Cases_on `h'` THEN Cases_on `p`  THEN METIS_TAC [APPEND, validStlItems, APPEND_ASSOC, APPEND_NIL]])
+Cases_on `h'` THEN Cases_on `p`  THEN 
+METIS_TAC [APPEND, validStlItems, APPEND_ASSOC, APPEND_NIL]]);
 
 
 val stackSyms_len = store_thm ("stackSyms_len", 
-``!stl.LENGTH stl = LENGTH (stackSyms stl)``,
-Induct_on `stl` THEN SRW_TAC [] [stackSyms_def] THEN
-FULL_SIMP_TAC (srw_ss()) [ADD1])
+``∀stl.LENGTH stl = LENGTH (stackSyms stl)``,
 
+Induct_on `stl` THEN FULL_SIMP_TAC (srw_ss()) [stackSyms_def, ADD1]);
 
 
 val auggr_notStartRule = store_thm ("auggr_notStartRule",
-``(slrmac ag = SOME m) ==> (validStates ag ((s, itl)::csl)) ==>
-(auggr g st eof = SOME ag) ==> ~(FST (FST (HD stl)) = TS eof) ==> 
-(?pfx.stackSyms stl = pfx++l) ==> 
-(getState m itl e = REDUCE (rule N l)) ==> ~(N=st)``,
+``(slrmac ag = SOME m) ⇒ (validStates ag ((s, itl)::csl)) ⇒
+(auggr g st eof = SOME ag) ⇒ ~(FST (FST (HD stl)) = TS eof) ⇒ 
+(∃pfx.stackSyms stl = pfx++l) ⇒ 
+(getState m itl e = REDUCE (rule N l)) ⇒ ~(N=st)``,
 SRW_TAC [] [] THEN 
 `MEM (rule N l) (rules ag)` by METIS_TAC [getstate_red, APPEND, validStates_def, sgoto_exp] THEN
 FULL_SIMP_TAC (srw_ss()) [stackSyms_def] THEN
@@ -206,8 +219,9 @@ SRW_TAC [] [] THEN METIS_TAC [auggr_neqStartSym],
 Cases_on `h` THEN Cases_on `q` THEN FULL_SIMP_TAC (srw_ss()) [] THEN
 Cases_on `l` THENL[
 SRW_TAC [] [] THEN METIS_TAC [auggr_neqStartSym],
-`LAST (REVERSE (MAP FST (MAP FST t)) ++ [q']) = LAST (pfx ++ h::t')` by METIS_TAC [] THEN
-METIS_TAC [auggr_neqStartSym2, last_elem, last_append, NOT_CONS_NIL]]])
+`LAST (REVERSE (MAP FST (MAP FST t)) ++ [q']) = LAST (pfx ++ h::t')` 
+		   by METIS_TAC [] THEN
+METIS_TAC [auggr_neqStartSym2, last_elem, last_append, NOT_CONS_NIL]]]);
 
 
 
@@ -216,192 +230,206 @@ val getState_nil = store_thm ("getState_nil",
 SRW_TAC [] [getState_def, LET_THM] THEN
 FULL_SIMP_TAC (srw_ss()) [] THEN
 Cases_on `sgoto g [] h` THEN 
-Cases_on `reduce g [] (sym2Str h)` THEN SRW_TAC [] [] THEN
-FULL_SIMP_TAC (srw_ss()) [reduce_def])
+Cases_on `reduce g [] (ts2str h)` THEN SRW_TAC [] [] THEN
+FULL_SIMP_TAC (srw_ss()) [reduce_def]);
 
 
 val reduce_mem_followSet = store_thm ("reduce_mem_followSet", 
-``!N r1 itl h.MEM (item N (r1,[])) itl ==> isTmnlSym h ==>
-h IN followSet ag (NTS N) ==> ~(reduce ag itl (sym2Str h) =[])``,
+``∀N r1 itl.MEM (item N (r1,[])) itl ⇒ isTmnlSym h ⇒
+h IN followSet ag (NTS N) ⇒ ~(reduce ag itl (ts2str h) =[])``,
+
 Induct_on `itl` THEN SRW_TAC [] [] THEN
 FULL_SIMP_TAC (srw_ss()) [reduce_def, LET_THM] THEN
-Cases_on `h'` THEN FULL_SIMP_TAC (srw_ss()) [sym2Str_def, followSetEq, isTmnlSym_def] THEN
+Cases_on `h` THEN FULL_SIMP_TAC (srw_ss()) [ts2str_def, followSetEq, 
+					     isTmnlSym_def] THEN
 RES_TAC THEN
-`~(reduce ag itl s = [])` by METIS_TAC [sym2Str_def] THEN
-Cases_on `h` THEN Cases_on `p` THEN 
-Cases_on `r` THEN FULL_SIMP_TAC (srw_ss()) [reduce_def, LET_THM , isTmnlSym_def, followSetEq] THEN
-Cases_on ` TS s IN followSet ag (NTS s')` THEN FULL_SIMP_TAC (srw_ss()) [])
+`~(reduce ag itl t = [])` by METIS_TAC [ts2str_def] THEN
+`reduce ag (h'::itl) t = reduce ag [h'] t ++ reduce ag itl t` 
+by METIS_TAC [reduce_append, APPEND] THEN
+FULL_SIMP_TAC (srw_ss()) []);
 
 
 
 val reduce_followSet = store_thm ("reduce_followSet",
-``!l s out.(reduce g l s = out) ==> (!e.MEM e out ==> (TS s) IN followSet g (NTS (ruleLhs e)))``,
+``∀l s out.(reduce g l s = out) ⇒ 
+(∀e.MEM e out ⇒ (TS s) IN followSet g (NTS (ruleLhs e)))``,
+
 Induct_on `l` THEN SRW_TAC [] [reduce_def] THEN
 FULL_SIMP_TAC (srw_ss()) [reduce_def] THEN
 Cases_on `h` THEN Cases_on `p` THEN Cases_on `r` THEN
 FULL_SIMP_TAC (srw_ss()) [reduce_def] THEN
-Cases_on `TS s IN followSetML g (NTS s')` THEN 
-FULL_SIMP_TAC (srw_ss()) [followSetEq, ruleLhs_def])
+Cases_on `TS s IN followSet g (NTS n)` THEN 
+FULL_SIMP_TAC (srw_ss()) [ruleLhs_def]);
 
 
 val getState_reduce_followSet = store_thm ("getState_reduce_followSet", 
-``(m=(sgoto g, reduce g)) ==> validItl g itl ==>
-isTmnlSym sym ==> (getState m itl sym = REDUCE (rule s' l)) ==> sym IN (followSet g (NTS s'))``,
+``(m=(sgoto g, reduce g)) ⇒ validItl g itl ⇒
+isTmnlSym sym ⇒ (getState m itl sym = REDUCE (rule s' l)) ⇒ 
+					   sym IN (followSet g (NTS s'))``,
+
 Cases_on `itl` THEN SRW_TAC [] [getState_def, LET_THM] THEN Cases_on `sym` THEN
-FULL_SIMP_TAC (srw_ss()) [isTmnlSym_def, sym2Str_def] THENL[
+FULL_SIMP_TAC (srw_ss()) [isTmnlSym_def, ts2str_def] 
+THENL[
 
-Cases_on `sgoto g [] (TS s)` THEN Cases_on `reduce g [] s` THEN FULL_SIMP_TAC (srw_ss()) [] THEN
+Cases_on `sgoto g [] (TS s)` THEN Cases_on `reduce g [] s` THEN 
+FULL_SIMP_TAC (srw_ss()) [] THEN
 FULL_SIMP_TAC (srw_ss()) [reduce_def],
 
-Cases_on `sgoto g [] (TS s)` THEN Cases_on `reduce g [] s` THEN FULL_SIMP_TAC (srw_ss()) [] THEN
+Cases_on `sgoto g [] (TS t)` THEN Cases_on `reduce g [] t` THEN 
+FULL_SIMP_TAC (srw_ss()) [] THEN
 FULL_SIMP_TAC (srw_ss()) [reduce_def],
 
 
-Cases_on `sgoto g (h::t) (TS s)` THEN Cases_on `reduce g (h::t) s` THEN
+Cases_on `sgoto g (h::t) (TS t')` THEN Cases_on `reduce g (h::t) t'` THEN
 FULL_SIMP_TAC (srw_ss()) [] THENL[
 SRW_TAC [] [] THEN
 METIS_TAC [ruleLhs_def, reduce_followSet, MEM],
-Cases_on `itemEqRuleList (h'::t') (h''::t'')` THEN FULL_SIMP_TAC (srw_ss()) [] THEN
+Cases_on `itemEqRuleList (h'::t'') (h''::t''')` THEN FULL_SIMP_TAC (srw_ss()) [] THEN
 METIS_TAC [ruleLhs_def, reduce_followSet, MEM]],
 
-Cases_on `sgoto g (h::t) (TS s)` THEN Cases_on `reduce g (h::t) s` THEN
+Cases_on `sgoto g (h::t) (TS t')` THEN Cases_on `reduce g (h::t) t'` THEN
 FULL_SIMP_TAC (srw_ss()) [] THEN
-Cases_on `itemEqRuleList (h'::t') (h''::t'')` THEN FULL_SIMP_TAC (srw_ss()) [] THEN
-METIS_TAC [ruleLhs_def, reduce_followSet, MEM]])
+Cases_on `itemEqRuleList (h'::t'') (h''::t''')` THEN 
+FULL_SIMP_TAC (srw_ss()) [] THEN
+METIS_TAC [ruleLhs_def, reduce_followSet, MEM]]);
 
 
 val validItls = Define `
 validItls ((s, itl)) topitl = 
-(!N r1 r2.(MEM (item N (r1,r2)) itl) ==> (r1=[]) \/
-(LAST r1 = s)) /\
-(!N' r1' r2'.(MEM (item N' (r1',r2')) topitl) ==> (r1'=[]) \/ (?l1 l2.(r1'=l1++[s]++l2) /\ 
+(∀N r1 r2.(MEM (item N (r1,r2)) itl) ⇒ (r1=[]) ∨
+(LAST r1 = s)) ∧
+(∀N' r1' r2'.(MEM (item N' (r1',r2')) topitl) ⇒ (r1'=[]) ∨ (∃l1 l2.(r1'=l1++[s]++l2) ∧ 
 MEM (item N' (l1++[s],l2++r2')) itl))`
 
 val stateValidItls = Define `
-(stateValidItls [] topitl = T) /\
-(stateValidItls (st::rst) topitl = validItls st topitl /\ stateValidItls rst topitl)`
+(stateValidItls [] topitl = T) ∧
+(stateValidItls (st::rst) topitl = validItls st topitl ∧ stateValidItls rst topitl)`;
 
-val symsAfterDot = Define `(symsAfterDot [] = []) /\
-(symsAfterDot (item l (r1,[])::t) = symsAfterDot t) /\
-(symsAfterDot (item l (r1,s::ss)::t) = s::symsAfterDot t)`
-
-
-val rhsEqItems = Define `rhsEqItems e1 e2 = (itemFstRhs e1 ++ itemSndRhs e1 = itemFstRhs e2 ++ itemSndRhs e2)`
+val symsAfterDot = Define `(symsAfterDot [] = []) ∧
+(symsAfterDot (item l (r1,[])::t) = symsAfterDot t) ∧
+(symsAfterDot (item l (r1,s::ss)::t) = s::symsAfterDot t)`;
 
 
-val isNewItem = Define `(isNewItem [] = T) /\
-(isNewItem ((item l (r1,r2))::rst) = if (r1=[]) then (isNewItem rst) else F)`
+val rhsEqItems = Define 
+`rhsEqItems e1 e2 = 
+(itemFstRhs e1 ++ itemSndRhs e1 = itemFstRhs e2 ++ itemSndRhs e2)`;
+
+
+val isNewItem = Define `(isNewItem [] = T) ∧
+(isNewItem ((item l (r1,r2))::rst) = if (r1=[]) then (isNewItem rst) else F)`;
 
 val isNewItem_rules2items = store_thm ("newItem_rules2items",
-``!g.isNewItem  (rules2Items (rules g))``,
+``∀g.isNewItem  (rules2Items (rules g))``,
 Cases_on `g` THEN SRW_TAC [] [rules_def] THEN
 Induct_on `l` THEN SRW_TAC [] [isNewItem, rules2Items_def] THEN
-Cases_on `h` THEN FULL_SIMP_TAC (srw_ss()) [isNewItem,rules2Items_def])
+Cases_on `h` THEN FULL_SIMP_TAC (srw_ss()) [isNewItem,rules2Items_def]);
 
 
 val isNewItem_append = store_thm ("isNewItem_append",
-``!l1 l2.isNewItem (l1++l2) = isNewItem l1 /\ isNewItem l2``,
+``∀l1 l2.isNewItem (l1++l2) = isNewItem l1 ∧ isNewItem l2``,
 Induct_on `l1` THEN Induct_on `l2` THEN SRW_TAC [] [isNewItem, EQ_IMP_THM] THEN
 Cases_on `h'` THEN Cases_on `p` THEN
-METIS_TAC [APPEND, isNewItem])
+METIS_TAC [APPEND, isNewItem]);
 
 
 val isNewItem_mem = store_thm ("isNewItem_mem",
-``!l. isNewItem l = (!e.MEM e l ==> isNewItem [e])``,
+``∀l. isNewItem l = (∀e.MEM e l ⇒ isNewItem [e])``,
 Induct_on `l` THEN SRW_TAC [] [isNewItem, EQ_IMP_THM] THEN
-METIS_TAC [isNewItem_append, APPEND])
+METIS_TAC [isNewItem_append, APPEND]);
+
 
 val isNewItem_getItems = store_thm ("isNewItem_getItems",
-``! g sym.isNewItem (getItems (rules g) sym)``,
-Induct_on `rules g` THEN SRW_TAC [] [isNewItem, getItems_def] THENL[
-METIS_TAC [isNewItem, getItems_def],
+``∀ g sym.isNewItem (getItems (rules g) sym)``,
+
+Induct_on `rules g` THEN SRW_TAC [] [isNewItem, getItems_def] THEN1
+METIS_TAC [isNewItem, getItems_def] THEN
 `rules g = h::v` by METIS_TAC [] THEN 
 Cases_on `h` THEN ONCE_ASM_REWRITE_TAC [] THEN
-`!e.MEM e (getItems (rule s l::v) sym) ==> MEM e (rules2Items (rule s l::v))` by METIS_TAC [rules2items_sub] THEN
-`isNewItem (rules2Items (rule s l ::v))` by METIS_TAC [isNewItem_rules2items, rules_def] THEN
-`!e.MEM e (rules2Items (rule s l::v)) ==> isNewItem [e]` by METIS_TAC [isNewItem_mem] THEN
-METIS_TAC [isNewItem_mem, APPEND, isNewItem_append, getItems_def]]) 
+`∀e.MEM e (getItems (rule n l::v) sym) ⇒ MEM e (rules2Items (rule n l::v))` by METIS_TAC [rules2items_sub] THEN
+`isNewItem (rules2Items (rule n l ::v))` by METIS_TAC [isNewItem_rules2items, rules_def] THEN
+`∀e.MEM e (rules2Items (rule n l::v)) ⇒ isNewItem [e]` by METIS_TAC [isNewItem_mem] THEN
+METIS_TAC [isNewItem_mem, APPEND, isNewItem_append, getItems_def]);
 
 
 val isNewItem_iclosure1 = store_thm ("isNewItem_iclosure1", 
-``!g itl.isNewItem itl ==> isNewItem (iclosure1 g itl)``,
+``∀g itl.isNewItem itl ⇒ isNewItem (iclosure1 g itl)``,
 Induct_on `itl` THEN SRW_TAC [] [isNewItem, iclosure1_def] THEN
 Cases_on `h` THEN Cases_on `p` THEN Cases_on `r` THEN
 FULL_SIMP_TAC (srw_ss()) [iclosure1_def, isNewItem] THEN
 Cases_on `h` THEN FULL_SIMP_TAC (srw_ss()) [iclosure1_def, isNewItem] THEN
-METIS_TAC [isNewItem, isNewItem_append, APPEND, APPEND_ASSOC, isNewItem_getItems])
+METIS_TAC [isNewItem, isNewItem_append, APPEND, APPEND_ASSOC, isNewItem_getItems]);
 
 
 val isNewItem_delete = store_thm ("isNewItem_delete",
-``!t h.isNewItem  t ==> isNewItem  (delete h t)``,
+``∀t h.isNewItem  t ⇒ isNewItem  (delete h t)``,
 Induct_on `t` THEN SRW_TAC [] [delete_def, isNewItem] THEN
-METIS_TAC [isNewItem_append, APPEND])
+METIS_TAC [isNewItem_append, APPEND]);
 
 
 val isNewItem_rmDupes = store_thm ("isNewItem_rmDupes", 
-``!itl.isNewItem  itl ==> isNewItem (rmDupes itl)``,
+``∀itl.isNewItem  itl ⇒ isNewItem (rmDupes itl)``,
 HO_MATCH_MP_TAC rmDupes_ind THEN SRW_TAC [] [rmDupes, isNewItem] THEN
-METIS_TAC [isNewItem_append, APPEND, isNewItem_delete])
+METIS_TAC [isNewItem_append, APPEND, isNewItem_delete]);
 
 
 val isNewItem_iclosure = store_thm ("isNewItem_iclosure",
-``!g itl.isNewItem  itl ==> isNewItem  (iclosure g itl)``,
+``∀g itl.isNewItem  itl ⇒ isNewItem  (iclosure g itl)``,
 HO_MATCH_MP_TAC iclosure_ind THEN SRW_TAC [] [iclosure, isNewItem, LET_THM] THEN
-METIS_TAC [isNewItem_rmDupes, isNewItem_iclosure1])
+METIS_TAC [isNewItem_rmDupes, isNewItem_iclosure1]);
 
 
 val isNewItem_initProds2Items = store_thm ("isNewItem_initProds2Items",
-``!s l.isNewItem (initProds2Items s l)``,
+``∀s l.isNewItem (initProds2Items s l)``,
 Induct_on `l` THEN SRW_TAC [] [initProds2Items_def, isNewItem] THEN
-Cases_on `h` THEN SRW_TAC [] [initProds2Items_def, isNewItem])
+Cases_on `h` THEN SRW_TAC [] [initProds2Items_def, isNewItem]);
 
 val isNewItem_everyNullFstRhs = store_thm ("isNewItem_everyNullFstRhs",
-``!l.isNewItem l = EVERY NULL (MAP itemFstRhs l)``,
+``∀l.isNewItem l = EVERY NULL (MAP itemFstRhs l)``,
 Induct_on `l` THEN SRW_TAC [] [isNewItem] THEN
 Cases_on `h` THEN  Cases_on `p` THEN
 FULL_SIMP_TAC (srw_ss()) [isNewItem, itemFstRhs_def] THEN
-METIS_TAC [NULL_EQ_NIL])
+METIS_TAC [NULL_EQ_NIL]);
 
 
 
 val b4DotEmpty = store_thm ("b4DotEmpty",
-``!g.(EVERY NULL (MAP itemFstRhs (initItems g (rules g))))``,
+``∀g.(EVERY NULL (MAP itemFstRhs (initItems g (rules g))))``,
 Cases_on `g` THEN
 SRW_TAC [] [rules_def] THEN
-Induct_on `l` THEN SRW_TAC [] [initItems_def, startSym_def, initProds2Items_def, iclosure] THEN
-METIS_TAC [isNewItem_everyNullFstRhs, isNewItem_initProds2Items, isNewItem_iclosure])
-
-
-
+Induct_on `l` THEN SRW_TAC [] [initItems_def, startSym_def, initProds2Items_def, 
+			       iclosure] THEN
+METIS_TAC [isNewItem_everyNullFstRhs, isNewItem_initProds2Items, 
+	   isNewItem_iclosure]);
 
 val nullFstRhs_validStlItems = store_thm ("nullFstRhs_validStlItems",
-``!l.(EVERY NULL (MAP itemFstRhs l)) ==> (validStlItems [] l)``,
+``∀l.(EVERY NULL (MAP itemFstRhs l)) ⇒ (validStlItems [] l)``,
 Induct_on `l` THEN SRW_TAC [] [validStlItems] THEN
 Cases_on `h` THEN Cases_on `p` THEN 
-FULL_SIMP_TAC (srw_ss()) [NULL_EQ_NIL, itemFstRhs_def, validStlItems, stackSyms_def, isSuffix_def, IS_PREFIX_REFL])
+FULL_SIMP_TAC (srw_ss()) [NULL_EQ_NIL, itemFstRhs_def, validStlItems,
+			  stackSyms_def, isSuffix_def, IS_PREFIX_REFL]);
 
 val validItl_initProds2Items = store_thm ("validItl_initProds2Items", 
-``!g l.validItl g (initProds2Items sym (rules g))``,
+``∀g l.validItl g (initProds2Items sym (rules g))``,
 Cases_on `g` THEN SRW_TAC [] [rules_def] THEN
 Induct_on `l` THEN SRW_TAC [] [initProds2Items_def, validItl_def, rules_def] THEN
 Cases_on `h` THEN
 SRW_TAC [] [initProds2Items_def, validItl_def, rules_def] THEN
-METIS_TAC [validItl_rules_cons])
+METIS_TAC [validItl_rules_cons]);
 
 
 val rderives_rules_cons = store_thm ("rderives_rules_cons", 
-``!s1 s2 r e.rderives (G r s) s1 s2 ==> rderives (G (e::r) s) s1 s2``,
+``∀s1 s2 r e.rderives (G r s) s1 s2 ⇒ rderives (G (e::r) s) s1 s2``,
 SRW_TAC [] [rderives_def, rules_def] THEN
-METIS_TAC [rules_def])
+METIS_TAC [rules_def]);
 
 
 val rtc_rderives_rules_cons = store_thm ("rtc_rderives_rules_cons", 
-``!s1 s2.RTC (rderives (G r s)) s1 s2 ==> RTC (rderives (G (e::r) s)) s1 s2``,
+``∀s1 s2.RTC (rderives (G r s)) s1 s2 ⇒ RTC (rderives (G (e::r) s)) s1 s2``,
 HO_MATCH_MP_TAC RTC_INDUCT THEN SRW_TAC [] [RTC_RULES] THEN
-METIS_TAC  [RTC_RULES, rderives_rules_cons])
+METIS_TAC  [RTC_RULES, rderives_rules_cons]);
 
 val validItem_rules_cons = store_thm ("validItem_rules_cons",
-``!r s l e.validItem (G r s) [] l ==> validItem (G (e::r) s) [] l``,
+``∀r s l e.validItem (G r s) [] l ⇒ validItem (G (e::r) s) [] l``,
 SRW_TAC [] [] THEN
 Induct_on `l` THEN SRW_TAC [] [validItem] THEN 
 Cases_on `p` THEN SRW_TAC [] [validItem, startSym_def] THEN
@@ -410,12 +438,13 @@ SRW_TAC [] [] THEN
 FULL_SIMP_TAC (srw_ss()) [] THEN
 Q.EXISTS_TAC `sfx` THEN
 SRW_TAC [] [rules_def] THEN
-METIS_TAC [rderives_rules_cons, rtc_rderives_rules_cons, rules_def])
+METIS_TAC [rderives_rules_cons, rtc_rderives_rules_cons, rules_def]);
 
 
 
 val validItem_initProds2Items = store_thm ("validItem_initProds2Items",
-``!g.EVERY (validItem g []) (initProds2Items (startSym g) (rules g))``,
+``∀g.EVERY (validItem g []) (initProds2Items (startSym g) (rules g))``,
+
 Cases_on `g` THEN 
 SRW_TAC [] [startSym_def, validItem, rules_def] THEN
 Induct_on `l` THEN SRW_TAC [] [initProds2Items_def] THEN
@@ -425,31 +454,30 @@ THENL[
       Q.EXISTS_TAC `[]`  THEN
       SRW_TAC [] [RTC_RULES] 
       THENL[
-	    MAP_EVERY Q.EXISTS_TAC [`[]`, `[]`, `l'`, `s`] THEN
+	    MAP_EVERY Q.EXISTS_TAC [`[]`, `[]`, `l'`, `n`] THEN
 	    SRW_TAC [] [rules_def],
 	    
 	    METIS_TAC [rules_def, MEM]
 	    ],
 
       METIS_TAC [validItem_rules_cons, EVERY_MEM],
-      METIS_TAC [validItem_rules_cons, EVERY_MEM]])
+      METIS_TAC [validItem_rules_cons, EVERY_MEM]]);
 
 
 val pfx_lem1 = prove(
-``!r1 e h t pfx t' sfx.
-(r1 ++ e :: h :: t = pfx ++ r1 ++ e :: t' ++ sfx) /\
-IS_PREFIX (pfx ++ r1 ++ e::t') r1 /\
-~(r1 = pfx ++ r1) ==>
+``∀r1 e h t pfx t' sfx.
+(r1 ++ e :: h :: t = pfx ++ r1 ++ e :: t' ++ sfx) ∧
+IS_PREFIX (pfx ++ r1 ++ e::t') r1 ∧
+~(r1 = pfx ++ r1) ⇒
 IS_PREFIX (pfx ++ r1 ++ e::t') (r1 ++ [e])``,
+
 Induct THEN SRW_TAC [][] THENL [
 Cases_on `pfx` THEN SRW_TAC [][] THEN
 FULL_SIMP_TAC (srw_ss()) [IS_PREFIX],
 
-Cases_on `pfx` THEN SRW_TAC [][] THENL [
-FULL_SIMP_TAC (srw_ss()) [],
-FULL_SIMP_TAC (srw_ss()) [] THENL [
-FULL_SIMP_TAC (srw_ss()) [],
-SRW_TAC [][IS_PREFIX] THEN
+Cases_on `pfx` THEN SRW_TAC [][] THEN
+FULL_SIMP_TAC (srw_ss()) [] THEN
+(SRW_TAC [][IS_PREFIX] THEN
 Q.MATCH_ABBREV_TAC `IS_PREFIX BIG SMALL` THEN
 `BIG = (t'' ++ [h]) ++ r1 ++ e::t'`
 by (SRW_TAC [][Abbr`BIG`] THEN
@@ -458,30 +486,28 @@ Q.UNABBREV_TAC `SMALL` THEN
 POP_ASSUM SUBST1_TAC THEN
 FIRST_X_ASSUM MATCH_MP_TAC THEN
 FULL_SIMP_TAC (srw_ss()) [IS_PREFIX] THEN
-METIS_TAC [APPEND_ASSOC, APPEND]]]]);
-
-
+METIS_TAC [APPEND_ASSOC, APPEND]) ]);
 
 
 
 val stateSym_stl_len1 = store_thm ("stateSym_stl_len1",
-``!stl.(MAP FST (MAP FST stl) = [NTS nt]) ==>
+``∀stl.(MAP FST (MAP FST stl) = [NTS nt]) ⇒
 (FST (FST (HD stl)) = NTS nt)``,
-Induct_on `stl` THEN SRW_TAC [] [])
+Induct_on `stl` THEN SRW_TAC [] []);
 
 
 val slrmacNotValid = store_thm ("slrmacNotValid",
-``MEM (item N (h,[])) itl ==> 
-(e IN (followSet ag (NTS N))) ==> (isTmnlSym e) ==>
-MEM (item N' (pfx,e::sfx)) itl ==> 
-(trans ag (initItems ag (rules ag),vp) = SOME itl) ==>
+``MEM (item N (h,[])) itl ⇒ 
+(e IN (followSet ag (NTS N))) ⇒ (isTmnlSym e) ⇒
+MEM (item N' (pfx,e::sfx)) itl ⇒ 
+(trans ag (initItems ag (rules ag),vp) = SOME itl) ⇒
 ~(slrmac ag = SOME (sgoto ag,reduce ag))``,
+
 SRW_TAC [] [slrmac_def, LET_THM] THEN
 FULL_SIMP_TAC (srw_ss()) [] THEN
-FIRST_X_ASSUM (Q.SPECL_THEN [`vp`,`itl`, `e`] ASSUME_TAC) THEN
-SRW_TAC [][] THEN
+MAP_EVERY Q.EXISTS_TAC [`vp`,`itl`,`e`] THEN SRW_TAC [][] THEN
 Cases_on `sgoto ag itl e` THEN
-Cases_on `reduce ag itl (sym2Str e)` THEN
+Cases_on `reduce ag itl (ts2str e)` THEN
 FULL_SIMP_TAC (srw_ss()) []
 THENL[
       METIS_TAC [reduce_not_mem],
@@ -492,26 +518,27 @@ THENL[
       METIS_TAC [reduce_not_mem],      
 
       Cases_on `t'` THEN FULL_SIMP_TAC (srw_ss()) []
-      ]
-)
+      ]);
 
 
 
-val stackTopSym = Define `stackTopSym stl = FST (FST (HD stl))`
+val stackTopSym = Define `stackTopSym stl = FST (FST (HD stl))`;
 
 
 val validItemNts = store_thm ("validItemNts",
-``!g p r.validItem g p (item l (r1,NTS nt::r2)) ==> 
-(!nt.nt IN (nonTerminals g) ==> gaw g nt) ==>
-MEM (rule nt r) (rules g) ==> validItem g p (item nt ([],r))``,
+``∀g p r.validItem g p (item l (r1,NTS nt::r2)) ⇒ 
+(∀nt.nt IN (nonTerminals g) ⇒ gaw g nt) ⇒
+MEM (rule nt r) (rules g) ⇒ validItem g p (item nt ([],r))``,
+
 SRW_TAC [] [validItem] THEN
 `(NTS nt)  IN (nonTerminals ( g))` by METIS_TAC [slemma1_4] THEN
 `~(language g = {})` by METIS_TAC [language_not_empty, slemma1_4] THEN
 `gaw g (NTS nt)` by METIS_TAC [language_def, gaw_def, slemma1_4] THEN
 FULL_SIMP_TAC (srw_ss()) [gaw_def] THEN
 `RTC (rderives g) [NTS nt] w` by METIS_TAC [derivesImpRderives] THEN
-Cases_on `([NTS nt] = w)` THEN SRW_TAC [] [] THEN FULL_SIMP_TAC (srw_ss()) [isTmnlSym_def] THEN
-`?sf.RTC (rderives g) [NTS nt] sf /\ rderives g sf w` by METIS_TAC [RTC_CASES2] THEN
+Cases_on `([NTS nt] = w)` THEN SRW_TAC [] [] THEN 
+FULL_SIMP_TAC (srw_ss()) [isTmnlSym_def] THEN
+`∃sf.RTC (rderives g) [NTS nt] sf ∧ rderives g sf w` by METIS_TAC [RTC_CASES2] THEN
 
 Cases_on `EVERY isTmnlSym (r2++sfx)` THENL[
 Q.EXISTS_TAC `r2++sfx` THEN SRW_TAC [] [] THENL[
@@ -524,12 +551,13 @@ METIS_TAC [rderives_append, APPEND_ASSOC]],
 `RTC (rderives ( g)) [NTS (startSym ( g))] (pfx ++ r1 ++ [NTS nt]++r2 ++ sfx)` by METIS_TAC [RTC_RULES_RIGHT1, APPEND, APPEND_ASSOC] THEN
 `gaw ( g) (NTS (startSym g))` by METIS_TAC [] THEN
 
-`?w.RTC (rderives g) (r2++sfx) w /\ EVERY isTmnlSym w` by 
-METIS_TAC [APPEND_ASSOC, APPEND, gaw_l1, gaw_def] THEN
+`∃w.RTC (rderives g) (r2++sfx) w ∧ EVERY isTmnlSym w` by 
+METIS_TAC [APPEND_ASSOC, APPEND,  gaw_def, rderivesImpDerives,gaw_l1] THEN
 
 `RTC (rderives ( g)) (pfx++r1++[NTS nt]++r2++sfx) (pfx++r1++[NTS nt]++w')` by 
 METIS_TAC [rtc_rderives_same_append_left, APPEND_ASSOC] THEN
- Cases_on `((pfx ++ r1 ++ [NTS nt] ++ r2 ++ sfx) = (pfx ++ r1 ++ [NTS nt] ++ w'))` THEN FULL_SIMP_TAC (srw_ss()) [] THENL[
+ Cases_on `((pfx ++ r1 ++ [NTS nt] ++ r2 ++ sfx) = (pfx ++ r1 ++ [NTS nt] ++ w'))` THEN 
+FULL_SIMP_TAC (srw_ss()) [] THENL[
 SRW_TAC [] [] THEN
 Q.EXISTS_TAC `w'` THEN SRW_TAC [] [] THEN
 METIS_TAC [rderives_append, APPEND_ASSOC, rdres1],
@@ -545,59 +573,60 @@ METIS_TAC [RTC_RTC, rderives_append, rdres1, APPEND_ASSOC],
 Q.EXISTS_TAC `w'` THEN SRW_TAC [] [] THEN
 `RTC (rderives g) (pfx ++ [NTS l] ++ sfx) (pfx ++ r1 ++ [NTS nt] ++ w')` by 
 METIS_TAC [RTC_SUBSET, RTC_RTC, APPEND, APPEND_ASSOC] THEN
-METIS_TAC [RTC_RTC, rderives_append, rdres1, APPEND_ASSOC]]])
+METIS_TAC [RTC_RTC, rderives_append, rdres1, APPEND_ASSOC]]]);
+
 
 
 val getItems_mem = store_thm ("getItems_mem",
-``!e l s'.MEM e (getItems l s') ==> ?r.(e=item s' ([],r)) /\ MEM (rule s' r) l``,
+``∀e l s'.MEM e (getItems l s') ⇒ ∃r.(e=item s' ([],r)) ∧ MEM (rule s' r) l``,
 Induct_on `l` THEN SRW_TAC [] [getItems_def] THEN
-Cases_on `h` THEN METIS_TAC [getItems_def, MEM])
+Cases_on `h` THEN METIS_TAC [getItems_def, MEM]);
 
 val validItem_getItems = store_thm ("validItem_getItems",
-``!g p s' t.validItem g p (item s (q,NTS s'::t)) ==> 
-(!nt.nt IN (nonTerminals g) ==> gaw g nt) ==>
+``∀g p s' t.validItem g p (item s (q,NTS s'::t)) ⇒ 
+(∀nt.nt IN (nonTerminals g) ⇒ gaw g nt) ⇒
 EVERY (validItem g p) (getItems (rules g) s')``,
 Induct_on `rules g` THEN SRW_TAC [] [] THENL[
 FULL_SIMP_TAC (srw_ss()) [getItems_def, validItem] THEN METIS_TAC [EVERY_DEF, getItems_def],
-`!e.MEM e (getItems (rules g) s') ==> ?r.(e=item s' ([],r)) /\ MEM (rule s' r) (rules g)` by METIS_TAC [getItems_mem] THEN
+`∀e.MEM e (getItems (rules g) s') ⇒ ∃r.(e=item s' ([],r)) ∧ MEM (rule s' r) (rules g)` by METIS_TAC [getItems_mem] THEN
 SRW_TAC [] [EVERY_MEM] THEN
 RES_TAC  THEN
 SRW_TAC [] [] THEN
-METIS_TAC [validItemNts]])
-
+METIS_TAC [validItemNts]]);
 
 
 val validItem_iclosure1 = store_thm ("validItem_iclosure1", 
-``!g itl l.EVERY (validItem g l) itl ==> 
-(!nt.nt IN (nonTerminals g) ==> gaw g nt) ==>
+``∀g itl l.EVERY (validItem g l) itl ⇒ 
+(∀nt.nt IN (nonTerminals g) ⇒ gaw g nt) ⇒
 EVERY (validItem g l) (iclosure1 g itl)``,
+
 Induct_on `itl` THEN SRW_TAC [] [iclosure1_def, validItem] THEN
 Cases_on `h` THEN Cases_on `p` THEN Cases_on `r` THEN
-FULL_SIMP_TAC (srw_ss()) [iclosure1_def, validItem] THENL[
-METIS_TAC [RTC_RULES],
-Cases_on `h` THEN SRW_TAC [] [iclosure1_def] THENL[
-SRW_TAC [] [validItem] THEN METIS_TAC [],
-`validItem g (pfx++q) (item s (q,NTS s'::t))` by METIS_TAC [validItem, APPEND_ASSOC] THEN
-METIS_TAC [validItem_getItems],
-`validItem g (pfx++q) (item s (q,NTS s'::t))` by METIS_TAC [validItem, APPEND_ASSOC] THEN
-METIS_TAC [validItem_getItems]]])
+FULL_SIMP_TAC (srw_ss()) [iclosure1_def, validItem] THEN1
+METIS_TAC [RTC_RULES] THEN
+Cases_on `h` THEN SRW_TAC [] [iclosure1_def] 
+THENL[
+      `validItem g (pfx++q) (item n (q,NTS n'::t))` by METIS_TAC [validItem, APPEND_ASSOC] THEN
+      METIS_TAC [validItem_getItems],
+      SRW_TAC [] [validItem] THEN METIS_TAC [],
+      SRW_TAC [] [validItem] THEN METIS_TAC []]);
 
 
 
 val validItem_delete = store_thm ("validItem_delete",
-``!t h.EVERY (validItem g l) t ==> EVERY (validItem g l) (delete h t)``,
-Induct_on `t` THEN SRW_TAC [] [delete_def, validItem])
+``∀t h.EVERY (validItem g l) t ⇒ EVERY (validItem g l) (delete h t)``,
+Induct_on `t` THEN SRW_TAC [] [delete_def, validItem]);
 
 
 val validItem_rmDupes = store_thm ("validItem_rmDupes", 
-``!itl g l.EVERY (validItem g l)  itl ==> EVERY (validItem g l) (rmDupes itl)``,
+``∀itl g l.EVERY (validItem g l)  itl ⇒ EVERY (validItem g l) (rmDupes itl)``,
 HO_MATCH_MP_TAC rmDupes_ind THEN SRW_TAC [] [rmDupes, validItem] THEN
-METIS_TAC [validItem_delete])
+METIS_TAC [validItem_delete]);
 
 
 val validItem_iclosure = store_thm ("validItem_iclosure",
-``!g itl l.EVERY (validItem g l)  itl ==> 
-(!nt.nt IN (nonTerminals g) ==> gaw g nt) ==>
+``∀g itl l.EVERY (validItem g l)  itl ⇒ 
+(∀nt.nt IN (nonTerminals g) ⇒ gaw g nt) ⇒
 EVERY (validItem g l)  (iclosure g itl)``,
 HO_MATCH_MP_TAC iclosure_ind THEN SRW_TAC [] [iclosure, validItem, LET_THM] THEN
 `EVERY (validItem g l) (v2::v3)` by FULL_SIMP_TAC (srw_ss()) [] THEN
@@ -606,37 +635,38 @@ HO_MATCH_MP_TAC iclosure_ind THEN SRW_TAC [] [iclosure, validItem, LET_THM] THEN
 by METIS_TAC [validItem_rmDupes, validItem_iclosure1, APPEND, EVERY_APPEND] THEN
 `EVERY (validItem g l) (rmDupes (iclosure1 g (rmDupes (v2::v3))))` 
 by METIS_TAC [validItem_rmDupes, validItem_iclosure1, APPEND, EVERY_APPEND] THEN
-METIS_TAC [])
+METIS_TAC []);
 
 
 
 val fstRhsNil_delete = store_thm ("fstRhsNil_delete",
-``!t h.EVERY NULL (MAP itemFstRhs t) ==> EVERY NULL (MAP itemFstRhs (delete h t))``,
-Induct_on `t` THEN SRW_TAC [] [delete_def])
+``∀t h.EVERY NULL (MAP itemFstRhs t) ⇒ EVERY NULL (MAP itemFstRhs (delete h t))``,
+Induct_on `t` THEN SRW_TAC [] [delete_def]);
 
 
 val fstRhsNil_rmDupes = store_thm ("fstRhsNil_rmDupes", 
-``!itl.EVERY NULL (MAP itemFstRhs itl) ==> EVERY NULL (MAP itemFstRhs (rmDupes itl))``,
+``∀itl.EVERY NULL (MAP itemFstRhs itl) ⇒ EVERY NULL (MAP itemFstRhs (rmDupes itl))``,
 HO_MATCH_MP_TAC rmDupes_ind THEN SRW_TAC [] [rmDupes] THEN
-METIS_TAC [APPEND, fstRhsNil_delete])
+METIS_TAC [APPEND, fstRhsNil_delete]);
 
 val every_map_itemFstRhs = store_thm ("every_map_itemFstRhs",
-``!l.EVERY NULL (MAP itemFstRhs l) = (!e.MEM e l ==> (itemFstRhs e = []))``,
+``∀l.EVERY NULL (MAP itemFstRhs l) = (∀e.MEM e l ⇒ (itemFstRhs e = []))``,
 Induct_on `l` THEN SRW_TAC [] [EQ_IMP_THM] THEN
 FULL_SIMP_TAC (srw_ss()) [] THEN
 Cases_on `e` THEN Cases_on `p` THEN
-FULL_SIMP_TAC (srw_ss()) [itemFstRhs_def, NULL_EQ_NIL])
+FULL_SIMP_TAC (srw_ss()) [itemFstRhs_def, NULL_EQ_NIL]);
 
 
 val fstRhsNil_getItems = store_thm ("fstRhsNil_getItems",
-``!l.EVERY NULL (MAP itemFstRhs (getItems l s'))``,
+``∀l.EVERY NULL (MAP itemFstRhs (getItems l s'))``,
+
 Induct_on `l` THEN SRW_TAC [] [getItems_def] THEN
 Cases_on `h` THEN FULL_SIMP_TAC (srw_ss()) [getItems_def] THEN
-Cases_on `s=s'` THEN FULL_SIMP_TAC (srw_ss()) [getItems_def, itemFstRhs_def])
+Cases_on `n=s'` THEN FULL_SIMP_TAC (srw_ss()) [getItems_def, itemFstRhs_def]);
 
 
 val fstRhsNil_iclosure1 = store_thm ("fstRhsNil_iclosure1",
-``!g l.EVERY NULL (MAP itemFstRhs l) ==> EVERY NULL (MAP itemFstRhs (iclosure1 g l))``,
+``∀g l.EVERY NULL (MAP itemFstRhs l) ⇒ EVERY NULL (MAP itemFstRhs (iclosure1 g l))``,
 Induct_on `l` THEN SRW_TAC [] [iclosure1_def] THEN
 Cases_on `h` THEN Cases_on `p` THEN 
 FULL_SIMP_TAC (srw_ss()) [itemFstRhs_def] THEN
@@ -644,10 +674,10 @@ FULL_SIMP_TAC (srw_ss()) [itemFstRhs_def] THEN
 SRW_TAC [] [] THEN
 Cases_on `r` THEN FULL_SIMP_TAC (srw_ss()) [iclosure1_def, itemFstRhs_def] THEN
 Cases_on `h` THEN FULL_SIMP_TAC (srw_ss()) [iclosure1_def, itemFstRhs_def] THEN
-METIS_TAC [fstRhsNil_getItems])
+METIS_TAC [fstRhsNil_getItems]);
 
 val fstRhsNil_iclosure = store_thm ("fstRhsNil_iclosure",
-``!g l.EVERY NULL (MAP itemFstRhs l) ==> MEM e (iclosure g l) ==> (itemFstRhs e=[])``,
+``∀g l.EVERY NULL (MAP itemFstRhs l) ⇒ MEM e (iclosure g l) ⇒ (itemFstRhs e=[])``,
 HO_MATCH_MP_TAC iclosure_ind THEN SRW_TAC [] [iclosure, iclosure1_def] THEN
 Cases_on `e` THEN Cases_on `p` THEN FULL_SIMP_TAC (srw_ss()) [itemFstRhs_def, LET_THM] THEN
 Cases_on `~(set (rmDupes (v2::v3)) =
@@ -663,84 +693,92 @@ METIS_TAC [fstRhsNil_iclosure1, fstRhsNil_rmDupes],
 Cases_on `r` THEN FULL_SIMP_TAC (srw_ss()) [rgr_r9eq] THEN SRW_TAC [] [] THEN
 POP_ASSUM MP_TAC THEN
 SRW_TAC [] [itemFstRhs_def] THEN
-METIS_TAC [NULL_EQ_NIL, NOT_CONS_NIL]])
-
-
+METIS_TAC [NULL_EQ_NIL, NOT_CONS_NIL]]);
 
 val fstRhsNil_initProds2Items = store_thm ("fstRhsNil_initProds2Items",
-``!l r1 r2. MEM (item l (r1,r2)) (initProds2Items s x) ==> (r1=[])``,
+``∀l r1 r2. MEM (item l (r1,r2)) (initProds2Items s x) ⇒ (r1=[])``,
+
 Induct_on `x` THEN SRW_TAC [] [] THEN
 FULL_SIMP_TAC (srw_ss()) [initProds2Items_def] THEN
 Cases_on `h` THEN Cases_on `r2` THEN 
 FULL_SIMP_TAC (srw_ss()) [initProds2Items_def] THEN
-Cases_on `s=s'` THEN FULL_SIMP_TAC (srw_ss()) [] THEN
-METIS_TAC [])
-
-
+Cases_on `n=s` THEN FULL_SIMP_TAC (srw_ss()) [] THEN
+METIS_TAC []);
 
 
 val initItems_fstRhs_nil = store_thm ("initItems_fstRhs_nil", 
-``!l r1 r2.MEM (item l (r1,r2)) (initItems ag (rules ag)) ==> (r1=[])``,
+``∀l r1 r2.MEM (item l (r1,r2)) (initItems ag (rules ag)) ⇒ (r1=[])``,
 SRW_TAC [] [initItems_def, initProds2Items_def] THEN
-`!l r1 r2.MEM (item l (r1,r2)) (initProds2Items (startSym ag) (rules ag)) ==> (r1 = [])` by 
+`∀l r1 r2.MEM (item l (r1,r2)) (initProds2Items (startSym ag) (rules ag)) ⇒ (r1 = [])` by 
 METIS_TAC [fstRhsNil_initProds2Items] THEN
 `EVERY NULL (MAP itemFstRhs (initProds2Items (startSym ag) (rules ag)))` by (FULL_SIMP_TAC (srw_ss()) [every_map_itemFstRhs] THEN
 SRW_TAC [] [] THEN Cases_on `e` THEN Cases_on `p` THEN
 FULL_SIMP_TAC (srw_ss()) [itemFstRhs_def] THEN METIS_TAC []) THEN
 `itemFstRhs (item l (r1,r2)) = []` by METIS_TAC [fstRhsNil_iclosure] THEN
-FULL_SIMP_TAC (srw_ss()) [itemFstRhs_def])
+FULL_SIMP_TAC (srw_ss()) [itemFstRhs_def]);
 
 
 val completeItem_sndRhs_nil = store_thm ("completeItem_sndRhs_nil",
-``!l r1 r2.MEM (item l (r1,r2)) (FILTER completeItem x) ==> (r2=[]) ``,
+``∀l r1 r2.MEM (item l (r1,r2)) (FILTER completeItem x) ⇒ (r2=[]) ``,
 Induct_on `x` THEN SRW_TAC [] [completeItem] THENL[
 Cases_on `r2` THEN FULL_SIMP_TAC (srw_ss()) [completeItem],
 METIS_TAC [],
-METIS_TAC []])
+METIS_TAC []]);
 
 
 val initProds_compItem_nil = store_thm ("initProds_compItem_nil", 
-``!l r1 r2.MEM (item l (r1, r2)) (FILTER completeItem (initItems ag (rules ag))) ==> ((r1=[]) /\ (r2=[]))``,
+``∀l r1 r2.MEM (item l (r1, r2)) (FILTER completeItem (initItems ag (rules ag))) ⇒ 
+					((r1=[]) ∧ (r2=[]))``,
 SRW_TAC [] [] THENL[
 METIS_TAC [MEM_FILTER, initItems_fstRhs_nil],
-METIS_TAC [completeItem_sndRhs_nil]])
+METIS_TAC [completeItem_sndRhs_nil]]);
 
 
 val mem_reduce = store_thm ("mem_reduce",
-``!e itl N.e IN followSet ag (NTS N) ==> MEM (item N (h,[])) itl ==> isTmnlSym e ==>
-    MEM (rule N h) (reduce ag itl (sym2Str e))``,
+``∀e itl N.e IN followSet ag (NTS N) ⇒ MEM (item N (h,[])) itl ⇒ isTmnlSym e ⇒
+    MEM (rule N h) (reduce ag itl (ts2str e))``,
+
 Induct_on `itl` THEN SRW_TAC [] [] THEN
 SRW_TAC [] [reduce_def] THEN
-Cases_on `e` THEN FULL_SIMP_TAC (srw_ss()) [sym2Str_def, isTmnlSym_def, followSetEq] THEN
-`reduce ag (h'::itl) s = reduce ag [h'] s ++ reduce ag itl s` by METIS_TAC [reduce_append, APPEND] THEN
+Cases_on `e` THEN FULL_SIMP_TAC (srw_ss()) [ts2str_def, isTmnlSym_def, followSetEq] THEN
+`reduce ag (h'::itl) t = reduce ag [h'] t ++ reduce ag itl t` by METIS_TAC [reduce_append, APPEND] THEN
 ONCE_ASM_REWRITE_TAC [] THEN
 SRW_TAC [] [] THEN
 RES_TAC THEN
-METIS_TAC [sym2Str_def])
+METIS_TAC [ts2str_def]);
+
+
+val isTmnlMemFollowSet = store_thm
+("isTmnlMemFollowSet",
+``e ∈ followSet ag (NTS N) ⇒ isTmnlSym e``,
+
+SRW_TAC [][followSet_def, isTmnlSym_def]);
 
 
 val slrmacCompItemsEq = 
 store_thm ("slrmacCompItemsEq",
-``!m ag N h itl.(SOME m = slrmac ag) ==> 
-(trans ag (initItems ag (rules ag),vp) = SOME itl) ==>
+``∀m ag N h itl.(SOME m = slrmac ag) ⇒ 
+(trans ag (initItems ag (rules ag),vp) = SOME itl) ⇒
                    MEM (item N (h,[])) itl 
-                ==> (e IN followSet ag (NTS N)) ==> isTmnlSym e ==>
-                (!j.
-                MEM j itl /\ completeItem j /\
-                e IN followSet ag (NTS (itemLhs j)) ==>
+                ⇒ (e IN followSet ag (NTS N)) ⇒
+                (∀j.
+                MEM j itl ∧ completeItem j ∧
+                e IN followSet ag (NTS (itemLhs j)) ⇒
                 (j = item N (h,[])))``,
+
 SRW_TAC [] [slrmac_def, LET_THM] THEN
 FULL_SIMP_TAC (srw_ss()) [] THEN
+`isTmnlSym e` by METIS_TAC [isTmnlMemFollowSet] THEN
 FIRST_X_ASSUM (Q.SPECL_THEN [`vp`,`itl`, `e`] ASSUME_TAC) THEN
 SRW_TAC [][] THEN
 FULL_SIMP_TAC (srw_ss()) [trans_def] THEN
 Cases_on `j=item N (h,[])` THEN
 SRW_TAC [] [] THEN
-`MEM (rule N h) (reduce ag itl (sym2Str e))` by METIS_TAC [mem_reduce] THEN
+`MEM (rule N h) (reduce ag itl (ts2str e))` by METIS_TAC [mem_reduce] THEN
 Cases_on `j` THEN 
 Cases_on `p` THEN Cases_on `r` THEN FULL_SIMP_TAC (srw_ss()) [completeItem, itemLhs_def] THEN
-`MEM (rule s q) (reduce ag itl (sym2Str e))` by METIS_TAC [mem_reduce] THEN
-Cases_on `sgoto ag itl e` THEN Cases_on `reduce ag itl (sym2Str e)` THEN 
+`MEM (rule N h) (reduce ag itl (ts2str e))` by METIS_TAC [mem_reduce] THEN
+Cases_on `sgoto ag itl e` THEN Cases_on `reduce ag itl (ts2str e)` THEN 
 FULL_SIMP_TAC (srw_ss()) [] THEN 
 REPEAT 
 (FULL_SIMP_TAC (srw_ss()) [] THEN 
@@ -752,19 +790,22 @@ REPEAT
 (Cases_on `t` THEN
 FULL_SIMP_TAC (srw_ss()) [] THEN
 (Cases_on `t'` THEN
-FULL_SIMP_TAC (srw_ss()) [])))
+FULL_SIMP_TAC (srw_ss()) [])) THEN
+Cases_on `t` THEN FULL_SIMP_TAC (srw_ss()) [] THEN
+SRW_TAC [][] THEN
+METIS_TAC [rule_11, mem_reduce, MEM]);
 
 
 
 val getItems_append = store_thm ("getItems_append",
-``!l1 l2.getItems (l1++l2) N  = getItems l1 N ++ getItems l2 N``,
+``∀l1 l2.getItems (l1++l2) N  = getItems l1 N ++ getItems l2 N``,
 Induct_on `l1` THEN Induct_on `l2` THEN SRW_TAC [] [getItems_def] THEN
-Cases_on `h'` THEN SRW_TAC [] [getItems_def])
+Cases_on `h'` THEN SRW_TAC [] [getItems_def]);
 
 
 val iclosureNt = store_thm ("iclosureNt",
-``!ag l.MEM (item lhs ([],NTS N::r2)) (iclosure ag l) ==> 
- !rhs.MEM (rule N rhs) (rules ag) ==>
+``∀ag l.MEM (item lhs ([],NTS N::r2)) (iclosure ag l) ⇒ 
+ ∀rhs.MEM (rule N rhs) (rules ag) ⇒
 MEM (item N ([],rhs)) (iclosure ag l)``,
 HO_MATCH_MP_TAC iclosure_ind THEN SRW_TAC [] [iclosure, LET_THM] THEN
 `(item lhs ([],NTS N::r2)) IN set (rmDupes (iclosure1 ag (rmDupes (v2::v3))))` by 
@@ -779,33 +820,33 @@ METIS_TAC [rmd_mem_list,containerLemmasTheory.mem_in]) THEN
 `MEM (item lhs ([],NTS N::r2)) (SET_TO_LIST (set (rmDupes (v2::v3))))` by 
 METIS_TAC [FINITE_LIST_TO_SET, MEM_SET_TO_LIST, SET_TO_LIST_IN_MEM] THEN
 `MEM (item lhs ([],NTS N::r2)) (rmDupes (v2::v3))` by METIS_TAC [stl_mem, FINITE_LIST_TO_SET] THEN
-`?p s.(rmDupes (v2::v3))=p++[item lhs ([],NTS N::r2)]++s`
+`∃p s.(rmDupes (v2::v3))=p++[item lhs ([],NTS N::r2)]++s`
     by METIS_TAC [rgr_r9eq] THEN
 FULL_SIMP_TAC (srw_ss()) [iclosure1_append,iclosure1_def] THEN
-`?r1 r2.rules ag=r1++[rule N rhs]++r2`
+`∃r1 r2.rules ag=r1++[rule N rhs]++r2`
     by METIS_TAC [rgr_r9eq] THEN
 FULL_SIMP_TAC (srw_ss()) [getItems_append,getItems_def] THEN
-METIS_TAC [rmd_mem_list,MEM,MEM_APPEND])
+METIS_TAC [rmd_mem_list,MEM,MEM_APPEND]);
 
 
 val initClosure = store_thm ("initClosure",
-``!l lhs r2.MEM (item lhs ([],NTS N::r2)) l ==> (l=(initItems ag (rules ag))) ==> 
- !rhs.MEM (rule N rhs) (rules ag) ==>
+``∀l lhs r2.MEM (item lhs ([],NTS N::r2)) l ⇒ (l=(initItems ag (rules ag))) ⇒ 
+ ∀rhs.MEM (rule N rhs) (rules ag) ⇒
 MEM (item N ([],rhs)) l``,
 SRW_TAC [] [initItems_def] THEN
 FULL_SIMP_TAC (srw_ss()) [initItems_def] THEN
-METIS_TAC [iclosureNt])
-
-
+METIS_TAC [iclosureNt]);
 
 
 val rtcImpInClosure = store_thm ("rtcImpInClosure",
-``!u u'.RTC (rderives ag) u u' ==> (u=[NTS (startSym ag)]) ==> !v.derives ag u' v ==>
-       (auggr g s eof = SOME ag) ==> (LENGTH v < LENGTH u' ==> isTmnlSym (HD u')) ==>
-        (?lhs r2.
+``∀u u'.RTC (rderives ag) u u' ⇒ (u=[NTS (startSym ag)]) ⇒ ∀v.derives ag u' v ⇒
+       (auggr g s eof = SOME ag) ⇒ (LENGTH v < LENGTH u' ⇒ isTmnlSym (HD u')) ⇒
+        (∃lhs r2.
       MEM (item lhs ([],HD v::r2))
         (initItems ag (rules ag)))``,
-HO_MATCH_MP_TAC RTC_STRONG_INDUCT_RIGHT1 THEN SRW_TAC [] [RTC_RULES] THENL[
+
+HO_MATCH_MP_TAC RTC_STRONG_INDUCT_RIGHT1 THEN SRW_TAC [] [RTC_RULES] 
+THENL[
 
 FULL_SIMP_TAC (srw_ss()) [lreseq, derives_def] THEN
 SRW_TAC [] [] THEN
@@ -846,7 +887,8 @@ SRW_TAC [] [] THEN
 Cases_on `s1` THEN SRW_TAC [] [] THEN
 FULL_SIMP_TAC (srw_ss()) [] THEN
 Cases_on `rhs` THEN SRW_TAC [] [] THEN
-FULL_SIMP_TAC (srw_ss()) [] THENL[
+FULL_SIMP_TAC (srw_ss()) [] 
+THENL[
 (* 4 subgoals *)
 Cases_on `s2` THEN FULL_SIMP_TAC (srw_ss()) [] THEN
 FULL_SIMP_TAC (srw_ss()) [derives_def],
@@ -874,12 +916,12 @@ Cases_on `s1` THEN FULL_SIMP_TAC (srw_ss()) [] THEN
 SRW_TAC [] [] THEN
 Cases_on `rhs` THEN FULL_SIMP_TAC (srw_ss()) [] THEN
 SRW_TAC [] [] THEN
-`derives ag (NTS lhs'::(t ++ [NTS lhs] ++ s2))  ((TS s''::t')++(t ++ [NTS lhs] ++ s2))` by METIS_TAC [res1, derives_same_append_right, APPEND] THEN
+`derives ag (NTS lhs'::(t ++ [NTS lhs] ++ s2))  ((TS s'::t')++(t ++ [NTS lhs] ++ s2))` by METIS_TAC [res1, derives_same_append_right, APPEND] THEN
 FULL_SIMP_TAC (srw_ss()) [derives_def] THEN
-`LENGTH (s1 ++ rhs ++ s2') = LENGTH (TS s''::(t' ++ t ++ [NTS lhs] ++ s2))` by METIS_TAC [] THEN
+`LENGTH (s1 ++ rhs ++ s2') = LENGTH (TS s'::(t' ++ t ++ [NTS lhs] ++ s2))` by METIS_TAC [] THEN
 FULL_SIMP_TAC (srw_ss()) [] THEN
 `~(SUC (LENGTH t' + LENGTH t + 1 + LENGTH s2) < SUC (LENGTH t) + 1 + LENGTH s2)` by DECIDE_TAC THEN
-FIRST_X_ASSUM (Q.SPECL_THEN [`(TS s''::(t' ++ t ++ [NTS lhs] ++ s2))`] MP_TAC) THEN
+FIRST_X_ASSUM (Q.SPECL_THEN [`(TS s'::(t' ++ t ++ [NTS lhs] ++ s2))`] MP_TAC) THEN
 SRW_TAC [] [] THEN
 METIS_TAC [],
 
@@ -891,12 +933,12 @@ Cases_on `s1` THEN FULL_SIMP_TAC (srw_ss()) [] THEN
 SRW_TAC [] [] THEN
 Cases_on `rhs` THEN FULL_SIMP_TAC (srw_ss()) [] THEN
 SRW_TAC [] [] THEN
-`derives ag (NTS lhs'::(t ++ [NTS lhs] ++ s2)) (TS s''::t''++(t ++ [NTS lhs] ++ s2))` by METIS_TAC [res1, derives_same_append_right, APPEND] THEN
+`derives ag (NTS lhs'::(t ++ [NTS lhs] ++ s2)) (TS s'::t''++(t ++ [NTS lhs] ++ s2))` by METIS_TAC [res1, derives_same_append_right, APPEND] THEN
 FULL_SIMP_TAC (srw_ss()) [derives_def] THEN
-`LENGTH (s1 ++ rhs ++ s2') = LENGTH (TS s''::(t'' ++ t ++ [NTS lhs] ++ s2))` by METIS_TAC [] THEN
+`LENGTH (s1 ++ rhs ++ s2') = LENGTH (TS s'::(t'' ++ t ++ [NTS lhs] ++ s2))` by METIS_TAC [] THEN
 FULL_SIMP_TAC (srw_ss()) [] THEN
 `~( SUC (LENGTH t'' + LENGTH t + 1 + LENGTH s2) < SUC (LENGTH t) + 1 + LENGTH s2)` by DECIDE_TAC THEN
-FIRST_X_ASSUM (Q.SPECL_THEN [`TS s''::(t'' ++ t ++ [NTS lhs] ++ s2)`] MP_TAC) THEN
+FIRST_X_ASSUM (Q.SPECL_THEN [`TS s'::(t'' ++ t ++ [NTS lhs] ++ s2)`] MP_TAC) THEN
 SRW_TAC [] [] THEN
 METIS_TAC []],
 
@@ -906,7 +948,8 @@ SRW_TAC [] [] THEN
 Cases_on `s1` THEN SRW_TAC [] [] THEN
 FULL_SIMP_TAC (srw_ss()) [] THEN
 Cases_on `rhs` THEN SRW_TAC [] [] THEN
-FULL_SIMP_TAC (srw_ss()) [] THENL[
+FULL_SIMP_TAC (srw_ss()) [] 
+THENL[
 (* 4 subgoals *)
 Cases_on `s2` THEN FULL_SIMP_TAC (srw_ss()) [] THEN
 FULL_SIMP_TAC (srw_ss()) [derives_def],
@@ -927,23 +970,23 @@ FIRST_X_ASSUM (Q.SPECL_THEN [`s2`, `[]`] MP_TAC) THEN
 SRW_TAC [] [] THEN
 METIS_TAC [initClosure],
 
-`derives ag (NTS lhs::s2) ((NTS s'::t)++s2)` by METIS_TAC [res1, derives_same_append_right, APPEND] THEN
+`derives ag (NTS lhs::s2) ((NTS n::t)++s2)` by METIS_TAC [res1, derives_same_append_right, APPEND] THEN
 FULL_SIMP_TAC (srw_ss()) [derives_def] THEN
 SRW_TAC [] [] THEN
-`LENGTH (s1 ++ rhs ++ s2'') = LENGTH (NTS s'::(t ++ s2))` by METIS_TAC [] THEN
+`LENGTH (s1 ++ rhs ++ s2'') = LENGTH (NTS n::(t ++ s2))` by METIS_TAC [] THEN
 FULL_SIMP_TAC (srw_ss()) [] THEN
 `~(SUC (LENGTH t + LENGTH s2) < 1 + LENGTH s2)` by DECIDE_TAC THEN
-FIRST_X_ASSUM (Q.SPECL_THEN [`NTS s'::(t ++ s2)`] MP_TAC) THEN
+FIRST_X_ASSUM (Q.SPECL_THEN [`NTS n::(t ++ s2)`] MP_TAC) THEN
 SRW_TAC [] [] THEN
 METIS_TAC [],
 
-`derives ag (NTS lhs::s2) ((NTS s'::t)++s2)` by METIS_TAC [res1, derives_same_append_right, APPEND] THEN
+`derives ag (NTS lhs::s2) ((NTS n::t)++s2)` by METIS_TAC [res1, derives_same_append_right, APPEND] THEN
 FULL_SIMP_TAC (srw_ss()) [derives_def] THEN
 SRW_TAC [] [] THEN
-`LENGTH (s1 ++ rhs ++ s2'') = LENGTH (NTS s'::(t ++ s2))` by METIS_TAC [] THEN
+`LENGTH (s1 ++ rhs ++ s2'') = LENGTH (NTS n::(t ++ s2))` by METIS_TAC [] THEN
 FULL_SIMP_TAC (srw_ss()) [] THEN
 `~(SUC (LENGTH t + LENGTH s2) < 1 + LENGTH s2)` by DECIDE_TAC THEN
-FIRST_X_ASSUM (Q.SPECL_THEN [`NTS s'::(t ++ s2)`] MP_TAC) THEN
+FIRST_X_ASSUM (Q.SPECL_THEN [`NTS n::(t ++ s2)`] MP_TAC) THEN
 SRW_TAC [] [] THEN
 METIS_TAC []],
 
@@ -966,12 +1009,12 @@ SRW_TAC [] [] THEN
 `~(1 + LENGTH t' < 1)` by DECIDE_TAC THEN
 METIS_TAC [],
 
-`derives ag  (NTS s'::(t ++ [NTS lhs] ++ s2)) (NTS s'::(t++s2))` by METIS_TAC [res1, derives_same_append_right, derives_same_append_left, APPEND_NIL, APPEND] THEN
+`derives ag  (NTS n::(t ++ [NTS lhs] ++ s2)) (NTS n::(t++s2))` by METIS_TAC [res1, derives_same_append_right, derives_same_append_left, APPEND_NIL, APPEND] THEN
 FULL_SIMP_TAC (srw_ss()) [derives_def] THEN
 SRW_TAC [] [] THEN
-FIRST_X_ASSUM (Q.SPECL_THEN [`NTS s'::(t' ++ [NTS lhs'] ++ s2')`] MP_TAC) THEN
+FIRST_X_ASSUM (Q.SPECL_THEN [`NTS n::(t' ++ [NTS lhs'] ++ s2')`] MP_TAC) THEN
 SRW_TAC [] [] THEN
-`LENGTH (s1 ++ rhs ++ s2'') = LENGTH (NTS s'::(t' ++ [NTS lhs'] ++ s2'))` by METIS_TAC [] THEN
+`LENGTH (s1 ++ rhs ++ s2'') = LENGTH (NTS n::(t' ++ [NTS lhs'] ++ s2'))` by METIS_TAC [] THEN
 FULL_SIMP_TAC (srw_ss()) [] THEN
 `~(SUC (LENGTH t' + 1 + LENGTH s2') <
              SUC (LENGTH t) + 1 + LENGTH s2)` by DECIDE_TAC THEN
@@ -980,15 +1023,15 @@ METIS_TAC [],
 `MEM (NTS lhs')  (t ++ s2)` by METIS_TAC [MEM_APPEND, rgr_r9eq] THEN
 FULL_SIMP_TAC (srw_ss()) [] THENL[
 
-`?pfx sfx.t=pfx++[NTS lhs']++sfx` by METIS_TAC [rgr_r9eq] THEN
+`∃pfx sfx.t=pfx++[NTS lhs']++sfx` by METIS_TAC [rgr_r9eq] THEN
 SRW_TAC [] [] THEN
-`derives ag (NTS s'::(pfx ++ [NTS lhs'] ++ sfx ++ [NTS lhs] ++ s2)) (NTS s'::(pfx ++ h::t'' ++ sfx)++ [NTS lhs] ++ s2)` by 
+`derives ag (NTS n::(pfx ++ [NTS lhs'] ++ sfx ++ [NTS lhs] ++ s2)) (NTS n::(pfx ++ h::t'' ++ sfx)++ [NTS lhs] ++ s2)` by 
 METIS_TAC [res1, derives_same_append_left, derives_same_append_right, APPEND, APPEND_ASSOC] THEN
 FULL_SIMP_TAC (srw_ss()) [derives_def] THEN
 SRW_TAC [] [] THEN
-FIRST_X_ASSUM (Q.SPECL_THEN [` NTS s'::(pfx ++ h::t'' ++ sfx ++ [NTS lhs] ++ s2)`] MP_TAC) THEN
+FIRST_X_ASSUM (Q.SPECL_THEN [` NTS n::(pfx ++ h::t'' ++ sfx ++ [NTS lhs] ++ s2)`] MP_TAC) THEN
 SRW_TAC [] [] THEN
-`LENGTH (s1 ++ rhs ++ s2'') = LENGTH (NTS s'::(pfx ++ h::t'' ++ sfx ++ [NTS lhs] ++ s2))` by METIS_TAC [] THEN
+`LENGTH (s1 ++ rhs ++ s2'') = LENGTH (NTS n::(pfx ++ h::t'' ++ sfx ++ [NTS lhs] ++ s2))` by METIS_TAC [] THEN
 FULL_SIMP_TAC (srw_ss()) [] THEN
 ` ~(SUC
  (LENGTH pfx + SUC (LENGTH t'') + LENGTH sfx + 1 +
@@ -996,15 +1039,15 @@ FULL_SIMP_TAC (srw_ss()) [] THEN
              SUC (LENGTH pfx + 1 + LENGTH sfx) + 1 + LENGTH s2)` by DECIDE_TAC THEN
 METIS_TAC [],
 
-`?pfx sfx.s2=pfx++[NTS lhs']++sfx` by METIS_TAC [rgr_r9eq] THEN
+`∃pfx sfx.s2=pfx++[NTS lhs']++sfx` by METIS_TAC [rgr_r9eq] THEN
 SRW_TAC [] [] THEN
-`derives ag (NTS s'::(t ++ [NTS lhs] ++ (pfx ++ [NTS lhs'] ++ sfx))) (NTS s'::(t ++ [NTS lhs] ++ (pfx ++ h::t'' ++ sfx)))` by 
+`derives ag (NTS n::(t ++ [NTS lhs] ++ (pfx ++ [NTS lhs'] ++ sfx))) (NTS n::(t ++ [NTS lhs] ++ (pfx ++ h::t'' ++ sfx)))` by 
 METIS_TAC [res1, derives_same_append_left, derives_same_append_right, APPEND, APPEND_ASSOC] THEN
 FULL_SIMP_TAC (srw_ss()) [derives_def] THEN
 SRW_TAC [] [] THEN
-FIRST_X_ASSUM (Q.SPECL_THEN [`NTS s'::(t ++ [NTS lhs] ++ pfx ++ h::t'' ++ sfx)`] MP_TAC) THEN
+FIRST_X_ASSUM (Q.SPECL_THEN [`NTS n::(t ++ [NTS lhs] ++ pfx ++ h::t'' ++ sfx)`] MP_TAC) THEN
 SRW_TAC [] [] THEN
-`LENGTH (s1 ++ rhs ++ s2) = LENGTH (NTS s'::(t ++ [NTS lhs] ++ pfx ++ h::t'' ++ sfx))` by METIS_TAC [] THEN
+`LENGTH (s1 ++ rhs ++ s2) = LENGTH (NTS n::(t ++ [NTS lhs] ++ pfx ++ h::t'' ++ sfx))` by METIS_TAC [] THEN
 FULL_SIMP_TAC (srw_ss()) [] THEN
 `~(SUC
                (LENGTH t + 1 + LENGTH pfx + SUC (LENGTH t'') + LENGTH sfx) <
@@ -1032,40 +1075,40 @@ FULL_SIMP_TAC (srw_ss()) [] THEN
 METIS_TAC [],
 
 
-`derives ag (NTS s'::(t ++ [NTS lhs] ++ s2)) (NTS s'::(t ++ (h'::t') ++ s2))` by METIS_TAC [res1, derives_same_append_right, derives_same_append_left, APPEND] THEN
+`derives ag (NTS n::(t ++ [NTS lhs] ++ s2)) (NTS n::(t ++ (h'::t') ++ s2))` by METIS_TAC [res1, derives_same_append_right, derives_same_append_left, APPEND] THEN
 FULL_SIMP_TAC (srw_ss()) [derives_def] THEN
 SRW_TAC [] [] THEN
-FIRST_X_ASSUM (Q.SPECL_THEN [`NTS s'::(t ++ h'::t' ++ s2)`] MP_TAC) THEN
+FIRST_X_ASSUM (Q.SPECL_THEN [`NTS n::(t ++ h'::t' ++ s2)`] MP_TAC) THEN
 SRW_TAC [] [] THEN
-`LENGTH (s1 ++ rhs ++ s2'') = LENGTH (NTS s'::(t ++ h'::t' ++ s2))` by METIS_TAC [] THEN
+`LENGTH (s1 ++ rhs ++ s2'') = LENGTH (NTS n::(t ++ h'::t' ++ s2))` by METIS_TAC [] THEN
 FULL_SIMP_TAC (srw_ss()) [] THEN
 `~(SUC (LENGTH t + SUC (LENGTH t') + LENGTH s2) <
              SUC (LENGTH t) + 1 + LENGTH s2)` by DECIDE_TAC THEN
 METIS_TAC [],
 
-`derives ag (NTS s'::(t ++ [NTS lhs] ++ s2)) (NTS s'::(t ++ (h'::t') ++ s2))` by METIS_TAC [res1, derives_same_append_right, derives_same_append_left, APPEND] THEN
+`derives ag (NTS n::(t ++ [NTS lhs] ++ s2)) (NTS n::(t ++ (h'::t') ++ s2))` by METIS_TAC [res1, derives_same_append_right, derives_same_append_left, APPEND] THEN
 FULL_SIMP_TAC (srw_ss()) [derives_def] THEN
 SRW_TAC [] [] THEN
-FIRST_X_ASSUM (Q.SPECL_THEN [`NTS s'::(t ++ h'::t' ++ s2)`] MP_TAC) THEN
+FIRST_X_ASSUM (Q.SPECL_THEN [`NTS n::(t ++ h'::t' ++ s2)`] MP_TAC) THEN
 SRW_TAC [] [] THEN
-`LENGTH (s1 ++ rhs ++ s2'') = LENGTH (NTS s'::(t ++ h'::t' ++ s2))` by METIS_TAC [] THEN
+`LENGTH (s1 ++ rhs ++ s2'') = LENGTH (NTS n::(t ++ h'::t' ++ s2))` by METIS_TAC [] THEN
 FULL_SIMP_TAC (srw_ss()) [] THEN
 `~(SUC (LENGTH t + SUC (LENGTH t') + LENGTH s2) <
              SUC (LENGTH t) + 1 + LENGTH s2)` by DECIDE_TAC THEN
-METIS_TAC []]]]]]])
+METIS_TAC []]]]]]]);
 
 
 
 val auggrLastEof = store_thm ("auggrLastEof",
-``(auggr g st eof = SOME ag) ==> 
-RTC (rderives ag) [NTS (startSym ag)] (h::pfx++[NTS N]++sfx) ==> ?pfx'. sfx = pfx' ++ [TS eof]``,
+``(auggr g st eof = SOME ag) ⇒ 
+RTC (rderives ag) [NTS (startSym ag)] (h::pfx++[NTS N]++sfx) ⇒ ∃pfx'. sfx = pfx' ++ [TS eof]``,
 SRW_TAC [] [Once RTC_CASES2, derives_def] THEN
 FULL_SIMP_TAC (srw_ss()) [rderives_def] THEN
 SRW_TAC [] [] THEN
 Cases_on `lhs=(startSym ag)` THEN SRW_TAC [] []
 THENL[
 
- `(s1=[]) /\ (s2=[])` by METIS_TAC [auggrRtcRderivesPfxSfxNil] THEN
+ `(s1=[]) ∧ (s2=[])` by METIS_TAC [auggrRtcRderivesPfxSfxNil] THEN
  SRW_TAC [] [] THEN
  FULL_SIMP_TAC (srw_ss()) [] THEN
  `rhs=[NTS (startSym g); TS eof]` by METIS_TAC [auggrStartRule] THEN
@@ -1078,7 +1121,7 @@ THENL[
  Cases_on `pfx` THEN FULL_SIMP_TAC (srw_ss()) []
  ],
  
- `?pfx'.s2=pfx'++[TS eof]` by METIS_TAC [lastEof] THEN
+ `∃pfx'.s2=pfx'++[TS eof]` by METIS_TAC [lastEof] THEN
  Cases_on `sfx` THEN SRW_TAC [] [] THEN
  FULL_SIMP_TAC (srw_ss()) [] 
  THENL[
@@ -1088,15 +1131,15 @@ THENL[
  `LAST [TS eof] = LAST (h'::t)` by METIS_TAC [last_append, NOT_CONS_NIL, APPEND_ASSOC, APPEND] THEN
  FULL_SIMP_TAC (srw_ss()) [] THEN
  METIS_TAC [APPEND_NIL, APPEND_FRONT_LAST, NOT_CONS_NIL]
- ]])
+ ]]);
 
 
 
 
 val initItemsHdNt = store_thm ("initItemsHdNt",
-``!u v.RTC (rderives ag) u v ==> (u=[NTS (startSym ag)]) ==> 
-   !N rst.(v=(NTS N::rst)) ==>
-   !rhs.MEM (rule N rhs) (rules ag) ==> (auggr g st eof = SOME ag) ==>
+``∀u v.RTC (rderives ag) u v ⇒ (u=[NTS (startSym ag)]) ⇒ 
+   ∀N rst.(v=(NTS N::rst)) ⇒
+   ∀rhs.MEM (rule N rhs) (rules ag) ⇒ (auggr g st eof = SOME ag) ⇒
     MEM (item N ([],rhs)) (initItems ag (rules ag))``,
 HO_MATCH_MP_TAC RTC_STRONG_INDUCT_RIGHT1 THEN SRW_TAC [] [RTC_RULES]
 THENL[
@@ -1112,13 +1155,13 @@ THENL[
       Cases_on `rhs'` THEN SRW_TAC [] [] THEN
       FULL_SIMP_TAC (srw_ss()) [isTmnlSym_def] THEN
       SRW_TAC [] [] THEN
-      METIS_TAC [initClosure]])
+      METIS_TAC [initClosure]]);
 
 
 val initItemsNtInBtwn = store_thm ("initItemsNtInBtwn",
-``!u v.RTC (rderives ag) u v ==> (u=[NTS (startSym ag)]) ==> !sl N rst.(v=sl++[NTS N]++rst) ==> ~(sl=[]) ==> EVERY isTmnlSym sl ==> 
+``∀u v.RTC (rderives ag) u v ⇒ (u=[NTS (startSym ag)]) ⇒ ∀sl N rst.(v=sl++[NTS N]++rst) ⇒ ~(sl=[]) ⇒ EVERY isTmnlSym sl ⇒ 
 (auggr g st eof = SOME ag)
- ==> ?lhs rhs.MEM (item lhs ([],HD (sl)::rhs)) (initItems ag (rules ag))``,
+ ⇒ ∃lhs rhs.MEM (item lhs ([],HD (sl)::rhs)) (initItems ag (rules ag))``,
 HO_MATCH_MP_TAC RTC_STRONG_INDUCT_RIGHT1 THEN SRW_TAC [] [RTC_RULES] THEN
 FULL_SIMP_TAC (srw_ss()) [lreseq] THEN
 Cases_on `sl` THEN SRW_TAC [] [] THEN
@@ -1133,7 +1176,7 @@ THENL[
       METIS_TAC [initItemsHdNt],
 
       SRW_TAC [] [] THEN
-      `(t'=t) \/ (?pfx sfx.(t'=t++[NTS N]++pfx) /\ (rst=pfx++sfx)) \/ (?pfx sfx.(t=pfx++sfx) /\ (t'=pfx))` by METIS_TAC [listCompLens]
+      `(t'=t) ∨ (∃pfx sfx.(t'=t++[NTS N]++pfx) ∧ (rst=pfx++sfx)) ∨ (∃pfx sfx.(t=pfx++sfx) ∧ (t'=pfx))` by METIS_TAC [listCompLens]
       THENL[
 	    SRW_TAC [] [] THEN
 	    FIRST_X_ASSUM (Q.SPECL_THEN [`TS s::t`] MP_TAC) THEN
@@ -1152,7 +1195,7 @@ THENL[
 	    ],
 
       SRW_TAC [] [] THEN
-      `(t'=t) \/ (?pfx sfx.(t'=t++[NTS N]++pfx) /\ (rst=pfx++sfx)) \/ (?pfx sfx.(t=pfx++sfx) /\ (t'=pfx))` by METIS_TAC [listCompLens, APPEND, APPEND_ASSOC, APPEND_NIL]
+      `(t'=t) ∨ (∃pfx sfx.(t'=t++[NTS N]++pfx) ∧ (rst=pfx++sfx)) ∨ (∃pfx sfx.(t=pfx++sfx) ∧ (t'=pfx))` by METIS_TAC [listCompLens, APPEND, APPEND_ASSOC, APPEND_NIL]
       THENL[
 
 	    SRW_TAC [] [] THEN
@@ -1170,28 +1213,28 @@ THENL[
 	    SRW_TAC [] [] THEN
 	    METIS_TAC [isTmnlSym_def, EVERY_DEF, APPEND_ASSOC, APPEND, NOT_CONS_NIL, HD, EVERY_APPEND]
 	    ]
-      ])
+      ]);
 
 
 
 val vsisLen = store_thm ("vsisLen",
-``!l1 l2.validStlItemsStack l1 l2 ==> (LENGTH l2 = LENGTH l1 + 1)``,
+``∀l1 l2.validStlItemsStack l1 l2 ⇒ (LENGTH l2 = LENGTH l1 + 1)``,
 Induct_on `l1` THEN Induct_on `l2` THEN SRW_TAC [] [] THEN
 FULL_SIMP_TAC (srw_ss()) [validStlItemsStack, validStlItems] THEN
 Cases_on `l2` THEN FULL_SIMP_TAC (srw_ss()) [validStlItemsStack, validStlItems] THEN
 Cases_on `l1` THEN FULL_SIMP_TAC (srw_ss()) [validStlItemsStack, validStlItems] THEN
-DECIDE_TAC)
+DECIDE_TAC);
 
 
 val validStlItems_pop_lemma = store_thm ("validStlItems_pop_lemma",
-``!h' t' h t n.validStlItemsStack (h'::t') (h::t) ==> validStlItemsStack (pop t' (n - 1)) (pop t (n - 1)) ==> 
+``∀h' t' h t n.validStlItemsStack (h'::t') (h::t) ⇒ validStlItemsStack (pop t' (n - 1)) (pop t (n - 1)) ⇒ 
 validStlItemsStack (pop (h'::t') n) (pop (h::t) n)``,
 Induct_on `n` THEN SRW_TAC [] [validStlItemsStack] THEN
 SRW_TAC [] [pop_def] THEN
-METIS_TAC [validStlItemsStack])
+METIS_TAC [validStlItemsStack]);
 
 val validStlItems_pop = store_thm("validStlItems_pop",
-``!l1 l2 n.validStlItemsStack l1 l2 ==> (n <= LENGTH l1) ==>
+``∀l1 l2 n.validStlItemsStack l1 l2 ⇒ (n <= LENGTH l1) ⇒
 validStlItemsStack (pop l1 n) (pop l2 n)``,
 Induct_on `l1` THEN Induct_on `l2` THEN SRW_TAC [] [validStlItemsStack] THEN
 Cases_on `l2` THEN FULL_SIMP_TAC (srw_ss()) [validStlItemsStack] THENL[
@@ -1204,7 +1247,7 @@ Cases_on `l1` THEN FULL_SIMP_TAC (srw_ss()) [validStlItemsStack]
 THENL[
 
  Cases_on `t` THEN FULL_SIMP_TAC (srw_ss()) [validStlItemsStack] THEN
- `(n=0) \/ (n=1)` by DECIDE_TAC THEN
+ `(n=0) ∨ (n=1)` by DECIDE_TAC THEN
  FULL_SIMP_TAC (srw_ss()) [pop_def, validStlItemsStack],
 
  `validStlItemsStack (h'''::t') (h''::t)` by METIS_TAC [validStlItemsStack] THEN
@@ -1212,17 +1255,17 @@ THENL[
  RES_TAC THEN
  `validStlItemsStack (h'::h'''::t') (h::h''::t)` by METIS_TAC [validStlItemsStack] THEN
 METIS_TAC [validStlItems_pop_lemma]
-]])
+]]);
 
 
 val rules2ItemsMemType = store_thm ("rules2ItemsMemType",
-``!l.MEM e (rules2Items l) ==> ?lhs r. e = item lhs ([],r)``,
+``∀l.MEM e (rules2Items l) ⇒ ∃lhs r. e = item lhs ([],r)``,
 Induct_on `l` THEN SRW_TAC [] [rules2Items_def] THEN
-Cases_on `h` THEN FULL_SIMP_TAC (srw_ss()) [rules2Items_def])
+Cases_on `h` THEN FULL_SIMP_TAC (srw_ss()) [rules2Items_def]);
 
 
 val iclosureMemNotMemList = store_thm ("iclosureMemNotMemList",
-``!g l.MEM e (iclosure g l) ==> ~MEM e l ==>  ?lhs r. (e = item lhs ([],r))``,
+``∀g l.MEM e (iclosure g l) ⇒ ~MEM e l ⇒  ∃lhs r. (e = item lhs ([],r))``,
 HO_MATCH_MP_TAC iclosure_ind THEN SRW_TAC [] [iclosure] THEN
 FULL_SIMP_TAC (srw_ss()) [LET_THM] THEN
 Cases_on ` ~(set (rmDupes (v2::v3)) =
@@ -1237,28 +1280,28 @@ THENL[
 
  `MEM e (rules2Items (rules g))` by METIS_TAC [iclosure1_outmem, rmd_r2, MEM] THEN
  METIS_TAC [rules2ItemsMemType]
- ])
+ ]);
 
 
 
 val sgotoMemType = store_thm ("sgotoMemType",
-``!e l itl.MEM e l ==> (l=(sgoto g itl h)) ==> (?lhs r.(e=item lhs ([],r)) \/ ?lhs r1 r2.(e=item lhs (r1++[h],r2)))``,
+``∀e l itl.MEM e l ⇒ (l=(sgoto g itl h)) ⇒ (∃lhs r.(e=item lhs ([],r)) ∨ ∃lhs r1 r2.(e=item lhs (r1++[h],r2)))``,
 Induct_on `itl` THEN SRW_TAC [] [] THEN
 FULL_SIMP_TAC (srw_ss()) [sgoto_def, nextState_def, moveDot_def, iclosure] THEN
 Cases_on `MEM e (moveDot (h'::itl) h)` THEN
-METIS_TAC [mdMem, iclosureMemNotMemList])
+METIS_TAC [mdMem, iclosureMemNotMemList]);
 
 
 val iclosureMemRhsFstNil = store_thm ("iclosureMemRhsFstNil",
-  ``!g l.~MEM (item lhs (r1 ++ [h],r2)) l ==> ~(MEM (item lhs (r1 ++ [h],r2)) (iclosure g l))``,
+  ``∀g l.~MEM (item lhs (r1 ++ [h],r2)) l ⇒ ~(MEM (item lhs (r1 ++ [h],r2)) (iclosure g l))``,
     SRW_TAC [] [] THEN
     Cases_on `~MEM (item lhs (r1 ++ [h],r2)) (iclosure g l)` THEN FULL_SIMP_TAC (srw_ss()) [] THEN
-    `?lhs' r. (item lhs (r1 ++ [h],r2)) = item lhs' ([],r)` by METIS_TAC [iclosureMemNotMemList] THEN
-    FULL_SIMP_TAC (srw_ss()) [])
+    `∃lhs' r. (item lhs (r1 ++ [h],r2)) = item lhs' ([],r)` by METIS_TAC [iclosureMemNotMemList] THEN
+    FULL_SIMP_TAC (srw_ss()) []);
 	      
 
 val sgotoMemItlType = store_thm ("sgotoMemItlType",
-``!itl l.MEM (item lhs (r1++[h],r2)) l ==>  (l=(sgoto g itl h)) ==> MEM (item lhs (r1,[h]++r2)) itl``,
+``∀itl l.MEM (item lhs (r1++[h],r2)) l ⇒  (l=(sgoto g itl h)) ⇒ MEM (item lhs (r1,[h]++r2)) itl``,
 Induct_on `itl` THEN SRW_TAC [] [] 
 THENL[
       Cases_on `l` THEN FULL_SIMP_TAC (srw_ss()) [sgoto_def, nextState_def, iclosure, moveDot_def],
@@ -1270,17 +1313,17 @@ THENL[
 	    FULL_SIMP_TAC (srw_ss()) [sgoto_def, nextState_def, iclosure, moveDot_def] THEN
 	    Cases_on `h=h'` THEN FULL_SIMP_TAC (srw_ss()) [] THEN
 	    SRW_TAC [] [] THEN
-	    `?l r1' r2'.
-	    ((item lhs (r1 ++ [h],r2)) = item l (r1' ++ [h],r2')) /\ MEM (item l (r1',h::r2')) itl` by METIS_TAC [mdMem] THEN
+	    `∃l r1' r2'.
+	    ((item lhs (r1 ++ [h],r2)) = item l (r1' ++ [h],r2')) ∧ MEM (item l (r1',h::r2')) itl` by METIS_TAC [mdMem] THEN
 	    FULL_SIMP_TAC (srw_ss()) [],
 	    
 	    METIS_TAC [iclosureMemRhsFstNil]
 	    ]
-      ])
+      ]);
 
 
 val vsis_cons = store_thm ("vsi_cons",
-``!h itl l el.validStlItemsStack l ((s,h::itl)::el) ==> validStlItemsStack l ((s,itl)::el)``,
+``∀h itl l el.validStlItemsStack l ((s,h::itl)::el) ⇒ validStlItemsStack l ((s,itl)::el)``,
 
 Induct_on `l` THEN SRW_TAC [] [validStlItemsStack] 
  THENL[
@@ -1288,15 +1331,15 @@ Induct_on `l` THEN SRW_TAC [] [validStlItemsStack]
  Cases_on `el` THEN FULL_SIMP_TAC (srw_ss()) [validStlItemsStack, validStlItems],
 
  FULL_SIMP_TAC (srw_ss()) [validStlItemsStack, validStlItems]
- ])
+ ]);
 
 val vsiAlt = store_thm ("vsiAlt",
-``!stl l.validStlItems stl l = (!e.MEM e l ==> isSuffix (itemFstRhs e) (stackSyms stl))``,
+``∀stl l.validStlItems stl l = (∀e.MEM e l ⇒ isSuffix (itemFstRhs e) (stackSyms stl))``,
 Induct_on `l` THEN SRW_TAC [] [EQ_IMP_THM, validStlItems] THEN
-FULL_SIMP_TAC (srw_ss()) [])
+FULL_SIMP_TAC (srw_ss()) []);
 
 val validStlItems_sgoto_gen = store_thm("validStlItems_sgoto_gen",
-``!l itl sym el l'.validStlItemsStack l ((s, itl)::el) ==> (l'=(sgoto g itl sym)) ==>
+``∀l itl sym el l'.validStlItemsStack l ((s, itl)::el) ⇒ (l'=(sgoto g itl sym)) ⇒
 validStlItems  (((sym, (sgoto g itl sym)),tr)::l) l'``,
 
 Induct_on `itl` THEN SRW_TAC [] [] 
@@ -1309,8 +1352,8 @@ Induct_on `itl` THEN SRW_TAC [] []
 FULL_SIMP_TAC (srw_ss()) [vsiAlt] THEN
 SRW_TAC [] [] THEN
 FULL_SIMP_TAC (srw_ss()) [stackSyms_def] THEN
-`?lhs r. 
-           (e = item lhs ([],r)) \/ ?lhs r1 r2. e = item lhs (r1 ++ [sym],r2)` by METIS_TAC [sgotoMemType] 
+`∃lhs r. 
+           (e = item lhs ([],r)) ∨ ∃lhs r1 r2. e = item lhs (r1 ++ [sym],r2)` by METIS_TAC [sgotoMemType] 
  THENL[
 
  SRW_TAC [] [isSuffix_def, IS_PREFIX, itemFstRhs_def],
@@ -1341,21 +1384,19 @@ Cases_on `l` THEN Cases_on `el` THEN FULL_SIMP_TAC (srw_ss()) [validStlItemsStac
  SRW_TAC [] [] THEN
  FULL_SIMP_TAC (srw_ss()) [validStlItems_append, validStlItems, stackSyms_def, isSuffix_def, itemFstRhs_def] THEN
  Cases_on `r1` THEN FULL_SIMP_TAC (srw_ss()) [REVERSE_APPEND, IS_PREFIX]
- ]]])
-
-
+ ]]]);
 
 
 val vsi_goto_lemma = store_thm ("vsi_goto_lemma",
-``!t itl l.validStlItems t itl ==>
-(!e.
-            MEM e l ==>
-            ?lhs r'.
-              (e = item lhs ([],r')) \/
-              ?lhs r1 r2. e = item lhs (r1 ++ [sym],r2)) ==>
-(!lhs r1 r2.
-            MEM (item lhs (r1 ++ [sym],r2)) l ==>
-            MEM (item lhs (r1,[sym] ++ r2)) itl) ==>
+``∀t itl l.validStlItems t itl ⇒
+(∀e.
+            MEM e l ⇒
+            ∃lhs r'.
+              (e = item lhs ([],r')) ∨
+              ∃lhs r1 r2. e = item lhs (r1 ++ [sym],r2)) ⇒
+(∀lhs r1 r2.
+            MEM (item lhs (r1 ++ [sym],r2)) l ⇒
+            MEM (item lhs (r1,[sym] ++ r2)) itl) ⇒
 validStlItems (((sym,l),tr)::t) l``,
 
 Induct_on `l` THEN SRW_TAC [] []  THENL[
@@ -1364,9 +1405,9 @@ SRW_TAC [] [validStlItems],
 
 SRW_TAC [] [validStlItems] THENL[
 
-`?lhs r'.
-              (h = item lhs ([],r')) \/
-              ?lhs r1 r2. h = item lhs (r1 ++ [sym],r2)` by METIS_TAC [] 
+`∃lhs r'.
+              (h = item lhs ([],r')) ∨
+              ∃lhs r1 r2. h = item lhs (r1 ++ [sym],r2)` by METIS_TAC [] 
 THENL[
 
 SRW_TAC [] [isSuffix_def, stackSyms_def, itemFstRhs_def, IS_PREFIX],
@@ -1378,7 +1419,7 @@ FULL_SIMP_TAC (srw_ss()) [validStlItems, isSuffix_def, itemFstRhs_def, IS_PREFIX
 ],
 
 
-Cases_on `~?e.MEM e l` THEN SRW_TAC [] [] THEN
+Cases_on `~∃e.MEM e l` THEN SRW_TAC [] [] THEN
 FULL_SIMP_TAC (srw_ss()) [] THENL[
 
 Cases_on `l` THEN FULL_SIMP_TAC (srw_ss()) [validStlItems] THEN
@@ -1392,26 +1433,26 @@ FULL_SIMP_TAC (srw_ss()) [] THEN
 FULL_SIMP_TAC (srw_ss()) [vsiAlt] THEN
 SRW_TAC [] [] THEN
 `isSuffix (itemFstRhs e') (stackSyms (((sym,l),tr)::t))` by METIS_TAC [] THEN
-FULL_SIMP_TAC (srw_ss()) [stackSyms_def]]]])
+FULL_SIMP_TAC (srw_ss()) [stackSyms_def]]]]);
 
 
 val validStlItems_goto = store_thm ("validStlItems_goto",
-``!g itl itl' sym t.(getState (sgoto g, reduce g) itl sym = GOTO itl') ==>
- validStlItems t itl ==>
-validStlItems (((sym,itl'), Leaf (sym2Str sym))::t) itl'``,
+``∀g itl itl' sym t.(getState (sgoto g, reduce g) itl sym = GOTO itl') ⇒
+ validStlItems t itl ⇒
+validStlItems (((sym,itl'), Leaf (ts2str sym))::t) itl'``,
 
 SRW_TAC [] [] THEN
 FULL_SIMP_TAC (srw_ss()) [getState_def, LET_THM] THEN
-Cases_on `sgoto g itl sym` THEN Cases_on `reduce g itl (sym2Str sym)` THEN FULL_SIMP_TAC (srw_ss()) [] 
+Cases_on `sgoto g itl sym` THEN Cases_on `reduce g itl (ts2str sym)` THEN FULL_SIMP_TAC (srw_ss()) [] 
  THENL[
  Cases_on `LENGTH t'=0` THEN FULL_SIMP_TAC (srw_ss()) [],
  
-`!e.MEM e (h::t') ==> ?lhs r'.(e = item lhs ([],r')) \/ ?lhs r1 r2. e = item lhs (r1 ++ [sym],r2)` by METIS_TAC [sgotoMemType, MEM] THEN
-`!lhs r1 r2.MEM (item lhs (r1 ++ [sym],r2)) (h::t') ==> MEM (item lhs (r1,[sym]++r2)) itl` by METIS_TAC [sgotoMemItlType, MEM] THEN
+`∀e.MEM e (h::t') ⇒ ∃lhs r'.(e = item lhs ([],r')) ∨ ∃lhs r1 r2. e = item lhs (r1 ++ [sym],r2)` by METIS_TAC [sgotoMemType, MEM] THEN
+`∀lhs r1 r2.MEM (item lhs (r1 ++ [sym],r2)) (h::t') ⇒ MEM (item lhs (r1,[sym]++r2)) itl` by METIS_TAC [sgotoMemItlType, MEM] THEN
 METIS_TAC [vsi_goto_lemma],
 
  Cases_on `itemEqRuleList (h::t') (h'::t'')` THEN FULL_SIMP_TAC (srw_ss()) []
- ])
+ ]);
 
 
 
@@ -1421,19 +1462,19 @@ validStates ag (state s itl::csl) = parse_csl_validStates
 *)
 
 val parse_validStlItemsStack = store_thm("parse_validStlItemsStack",
-``!m g.validStlItemsStack stl csl ==> (m=slrmac g) ==>
-~NULL csl ==> (* preserved by parse_csl_not_nil *)
-(LENGTH csl = LENGTH stl + 1) ==> (* another invariant *)
-EVERY (\x.~(x=[])) (MAP SND csl) ==> (* prove this as an invariant!!!!! *)
-~(stl=[]) ==>
-(parse m (sl, stl, csl) = SOME (sl',stl',csl')) ==> validStlItems stl' (SND (HD csl'))``,
+``∀m g.validStlItemsStack stl csl ⇒ (m=slrmac g) ⇒
+~NULL csl ⇒ (* preserved by parse_csl_not_nil *)
+(LENGTH csl = LENGTH stl + 1) ⇒ (* another invariant *)
+EVERY (\x.~(x=[])) (MAP SND csl) ⇒ (* prove this as an invariant∀∀∀∀∀ *)
+~(stl=[]) ⇒
+(parse m (sl, stl, csl) = SOME (sl',stl',csl')) ⇒ validStlItems stl' (SND (HD csl'))``,
 
 SRW_TAC [] [] THEN
-`?x y.csl = x::y` by METIS_TAC [list_mem2, NULL_EQ_NIL] THEN
+`∃x y.csl = x::y` by METIS_TAC [list_mem2, NULL_EQ_NIL] THEN
 SRW_TAC [] [] THEN
 Cases_on `x` THEN
 `~NULL csl'` by METIS_TAC [parse_csl_not_nil] THEN
-`?x' y'.csl' = x'::y'` by (Induct_on `csl'` THEN SRW_TAC [] []) THEN
+`∃x' y'.csl' = x'::y'` by (Induct_on `csl'` THEN SRW_TAC [] []) THEN
 SRW_TAC [] [] THEN
 FULL_SIMP_TAC (srw_ss()) [parse_def, LET_THM] THEN 
 Cases_on `slrmac g ` THEN  Cases_on `sl` THEN FULL_SIMP_TAC (srw_ss()) [] THEN
@@ -1454,7 +1495,7 @@ FULL_SIMP_TAC (srw_ss()) [ruleLhs_def, ruleRhs_def] THEN
 Cases_on `r` THEN FULL_SIMP_TAC (srw_ss()) [] THEN
 FULL_SIMP_TAC (srw_ss()) [ADD1] THEN
 `x=(sgoto g, reduce g)` by METIS_TAC [sgoto_exp] THEN FULL_SIMP_TAC (srw_ss()) [] THEN
-`?e el.(pop ((q, (h''::t'))::y) (LENGTH l)) = e::el` by METIS_TAC [list_nchotomy] THEN
+`∃e el.(pop ((q, (h''::t'))::y) (LENGTH l)) = e::el` by METIS_TAC [list_nchotomy] THEN
 FULL_SIMP_TAC (srw_ss()) [] THEN
 `LENGTH (h'::t) >= LENGTH l` by METIS_TAC [addrule_len] THEN
 `LENGTH l <= LENGTH (h'::t)` by DECIDE_TAC THEN
@@ -1482,7 +1523,7 @@ FULL_SIMP_TAC (srw_ss()) [ruleLhs_def, ruleRhs_def] THEN
 Cases_on `r` THEN FULL_SIMP_TAC (srw_ss()) [] THEN
 FULL_SIMP_TAC (srw_ss()) [ADD1] THEN
 `x=(sgoto g, reduce g)` by METIS_TAC [sgoto_exp] THEN FULL_SIMP_TAC (srw_ss()) [] THEN
-`?e el.(pop ((q, (h'::t'))::y) (LENGTH l)) = e::el` by METIS_TAC [list_nchotomy] THEN
+`∃e el.(pop ((q, (h'::t'))::y) (LENGTH l)) = e::el` by METIS_TAC [list_nchotomy] THEN
 FULL_SIMP_TAC (srw_ss()) [] THEN
 `LENGTH (h''::t) >= LENGTH l` by METIS_TAC [addrule_len] THEN
 `LENGTH l <= LENGTH (h''::t)` by DECIDE_TAC THEN
@@ -1513,11 +1554,11 @@ FULL_SIMP_TAC (srw_ss()) [push_def,validStlItemsStack] THEN
 SRW_TAC [] [] THEN
 `x=(sgoto g, reduce g)` by METIS_TAC [sgoto_exp] THEN
 SRW_TAC [] [] THEN
-METIS_TAC [sgoto_exp, validStlItems_goto, APPEND, APPEND_ASSOC, validStlItems]])
+METIS_TAC [sgoto_exp, validStlItems_goto, APPEND, APPEND_ASSOC, validStlItems]]);
 
 
 val validItem_moveDot = store_thm ("validItem_moveDot",
-``!itl.EVERY (validItem ag p) itl ==>
+``∀itl.EVERY (validItem ag p) itl ⇒
 EVERY (validItem ag (p++[h])) (moveDot itl h)``,
 Induct_on `itl` THEN SRW_TAC [] [moveDot_def] THEN
 Cases_on `h'` THEN Cases_on `p'` THEN
@@ -1525,43 +1566,44 @@ Cases_on `r` THEN FULL_SIMP_TAC (srw_ss()) [moveDot_def]  THEN
 Cases_on `h'=h` THEN FULL_SIMP_TAC (srw_ss()) [] THEN
 FULL_SIMP_TAC (srw_ss()) [validItem] THEN
 SRW_TAC [] [] THEN
-METIS_TAC [APPEND, APPEND_ASSOC])
+METIS_TAC [APPEND, APPEND_ASSOC]);
 
 
 
 val getState_reduce_not_NA = store_thm ("getState_reduce_not_NA", 
-``!N r1 itl h ag. 
-(slrmac ag = SOME (sgoto ag, reduce ag)) ==> 
-(trans ag (initItems ag (rules ag),vp) = SOME itl) ==>
-MEM (item N (r1,[])) itl ==>
- h IN followSet ag (NTS N) ==> isTmnlSym h ==>
-(!j.
-             MEM j itl /\ completeItem j /\
-             h IN followSet ag (NTS (itemLhs j)) ==>
+``∀N r1 itl h ag. 
+(slrmac ag = SOME (sgoto ag, reduce ag)) ⇒ 
+(trans ag (initItems ag (rules ag),vp) = SOME itl) ⇒
+MEM (item N (r1,[])) itl ⇒
+ h IN followSet ag (NTS N) ⇒ isTmnlSym h ⇒
+(∀j.
+             MEM j itl ∧ completeItem j ∧
+             h IN followSet ag (NTS (itemLhs j)) ⇒
              (j = item N (r1,[])))
-==> ~(getState (sgoto ag,reduce ag) itl h = NA)``,
+⇒ ~(getState (sgoto ag,reduce ag) itl h = NA)``,
+
 SRW_TAC [] [] THEN
 FULL_SIMP_TAC (srw_ss()) [slrmac_def, LET_THM] THEN
-Cases_on `?pfx itl' sym.
-               (trans ag (initItems ag (rules ag),pfx) = SOME itl') /\
+Cases_on `∃pfx itl' sym. isTmnlSym sym ∧
+               (trans ag (initItems ag (rules ag),pfx) = SOME itl') ∧
                case sgoto ag itl' sym of
                   [] ->
-                    (case reduce ag itl' (sym2Str sym) of
+                    (case reduce ag itl' (ts2str sym) of
                         [] -> F
                      || [v12] -> F
                      || v12::v16::v17 -> T)
                || v8::v9 ->
-                    case reduce ag itl' (sym2Str sym) of
+                    case reduce ag itl' (ts2str sym) of
                        [] -> F
                     || [v20] -> T
                     || v20::v26::v27 -> T` THEN 
-FULL_SIMP_TAC (srw_ss()) [] THEN
+(FULL_SIMP_TAC (srw_ss()) [] THEN
 FIRST_X_ASSUM (Q.SPECL_THEN [`vp`,`itl`,`h`] MP_TAC) THEN
 SRW_TAC [][] THEN
 FULL_SIMP_TAC (srw_ss()) [] THEN
 FULL_SIMP_TAC (srw_ss()) [getState_def, LET_THM] THEN
 Cases_on `sgoto ag itl h` THEN 
-Cases_on `reduce ag itl (sym2Str h)` THEN
+Cases_on `reduce ag itl (ts2str h)` THEN
 FULL_SIMP_TAC (srw_ss()) [] THENL[
 METIS_TAC [reduce_mem_followSet, NOT_CONS_NIL],
 
@@ -1571,18 +1613,21 @@ FULL_SIMP_TAC (srw_ss()) [],
 
 Cases_on `itemEqRuleList (h'::t) (h''::t')` THEN SRW_TAC [] [] THEN
 FULL_SIMP_TAC (srw_ss()) [] THEN
-Cases_on `t'` THEN FULL_SIMP_TAC (srw_ss()) []])
+Cases_on `t'` THEN FULL_SIMP_TAC (srw_ss()) []]));
 
 
 
-val getState_shift_not_NA = store_thm ("getState_shift_not_NA",
-``!g N r1 h' t itl.(SOME (sgoto g, reduce g) = slrmac g) ==>
-MEM (item N (r1,h'::t)) itl ==> 
-(trans g (initItems g (rules g),vp) = SOME itl) ==>
+val getState_shift_not_NA = store_thm 
+("getState_shift_not_NA",
+``∀g N r1 h' t itl.(SOME (sgoto g, reduce g) = slrmac g) ⇒
+MEM (item N (r1,h'::t)) itl ⇒ isTmnlSym h' ⇒
+(trans g (initItems g (rules g),vp) = SOME itl) ⇒
 ~(getState (sgoto g, reduce g) itl h' = NA)``,
+
 SRW_TAC [] [] THEN
 FULL_SIMP_TAC (srw_ss()) [getState_def, LET_THM] THEN
-Cases_on `sgoto g itl h'` THEN Cases_on `reduce g itl (sym2Str h')` THEN FULL_SIMP_TAC (srw_ss()) [] 
+Cases_on `sgoto g itl h'` THEN 
+Cases_on `reduce g itl (ts2str h')` THEN FULL_SIMP_TAC (srw_ss()) [] 
 THENL[
       METIS_TAC [sgoto_mem, NOT_CONS_NIL, APPEND, MEM, rgr_r9eq],
 
@@ -1590,35 +1635,36 @@ THENL[
 
       Cases_on `itemEqRuleList (h::t') (h''::t'')` THEN SRW_TAC [] [] THEN
       FULL_SIMP_TAC (srw_ss()) [slrmac_def, LET_THM] THEN
-      Cases_on `?pfx itl' sym.
-               (trans g (initItems g (rules g),pfx) = SOME itl') /\
+      Cases_on `∃pfx itl' sym. isTmnlSym sym ∧
+               (trans g (initItems g (rules g),pfx) = SOME itl') ∧
                case sgoto g itl' sym of
                   [] ->
-                    (case reduce g itl' (sym2Str sym) of
+                    (case reduce g itl' (ts2str sym) of
                         [] -> F
                      || [v12] -> F
                      || v12::v16::v17 -> T)
                || v8::v9 ->
-                    case reduce g itl' (sym2Str sym) of
+                    case reduce g itl' (ts2str sym) of
                        [] -> F
                     || [v20] -> T
                     || v20::v26::v27 -> T` THEN 
       FULL_SIMP_TAC (srw_ss()) [] THEN
       FIRST_X_ASSUM (Q.SPECL_THEN [`vp`,`itl`, `h'`] MP_TAC) THEN
       SRW_TAC [][] THEN
-      Cases_on `t''` THEN SRW_TAC [][]])
+      Cases_on `t''` THEN SRW_TAC [][]]);
 
-
-
-val validStkSymTree_stateSym_eq_ptree2Sym = store_thm ("validStkSymTree_stateSym_eq_ptree2Sym", 
-``!stl.validStkSymTree stl ==> ((MAP FST (MAP FST stl)) = (MAP (ptree2Sym o SND) stl))``,
+val validStkSymTree_stateSym_eq_ptree2Sym = store_thm 
+("validStkSymTree_stateSym_eq_ptree2Sym", 
+``∀stl.validStkSymTree stl ⇒ ((MAP FST (MAP FST stl)) = (MAP (ptree2Sym o SND) stl))``,
 Induct_on `stl` THEN SRW_TAC [] [] THEN
 Cases_on `h` THEN Cases_on `q` THEN Cases_on `r` THEN
-FULL_SIMP_TAC (srw_ss()) [ptree2Sym_def, validStkSymTree_def])
+FULL_SIMP_TAC (srw_ss()) [ptree2Sym_def, validStkSymTree_def]);
 
 
 val addRule_SOME = store_thm ("addRule_SOME",
-``!pfx l stl.(stackSyms stl = pfx++l) ==> validStkSymTree stl ==> ?x.(addRule stl (rule N l) = SOME x)``,
+``∀pfx l stl.(stackSyms stl = pfx++l) ⇒ validStkSymTree stl 
+			      ⇒ ∃x.(addRule stl (rule N l) = SOME x)``,
+
 SRW_TAC [] [] THEN
 FULL_SIMP_TAC (srw_ss()) [buildTree_def, LET_THM, stackSyms_def, addRule_def] THEN
 `((MAP FST (MAP FST stl)) = (MAP (ptree2Sym o SND) stl))` by METIS_TAC [validStkSymTree_stateSym_eq_ptree2Sym] THEN
@@ -1630,34 +1676,36 @@ FULL_SIMP_TAC (srw_ss()) [] THEN
 `LENGTH l + LENGTH pfx >= LENGTH l` by DECIDE_TAC THEN
 `LENGTH (REVERSE l) + LENGTH (REVERSE pfx) >= LENGTH (REVERSE l)` by DECIDE_TAC THEN
 `LENGTH (REVERSE l ++ REVERSE pfx) >= (LENGTH (REVERSE l))` by FULL_SIMP_TAC (srw_ss()) [] THEN
-`?x.((take (LENGTH (REVERSE l)) (REVERSE l ++ REVERSE pfx)) = SOME x)` by METIS_TAC [take_valid] THEN
+`∃x.((take (LENGTH (REVERSE l)) (REVERSE l ++ REVERSE pfx)) = SOME x)` by METIS_TAC [take_valid] THEN
 FULL_SIMP_TAC (srw_ss()) [] THEN
-Cases_on `l` THEN SRW_TAC [] [] THEN FULL_SIMP_TAC (srw_ss()) [] THENL[
-FULL_SIMP_TAC (srw_ss()) [take_def, take10] THEN
-SRW_TAC [] [] THEN
-FULL_SIMP_TAC (srw_ss()) [],
-SRW_TAC [] [] THEN FULL_SIMP_TAC (srw_ss()) [] THEN FULL_SIMP_TAC (arith_ss) [] THEN
-`~((LENGTH (REVERSE t) + 1) = 0)` by DECIDE_TAC THEN
-`LENGTH (REVERSE t ++ [h]) = (LENGTH (REVERSE t) + 1)` by FULL_SIMP_TAC (arith_ss) [rev_nil, LENGTH, LENGTH_APPEND] THEN
-`take (LENGTH (REVERSE t) + 1) (REVERSE t ++ [h] ++ REVERSE pfx) = SOME (REVERSE t ++ [h])` by METIS_TAC [takenthm] THEN
-FULL_SIMP_TAC (srw_ss()) [] THEN
-`LENGTH (MAP SND stl) = LENGTH (x ++ REVERSE pfx)` by METIS_TAC [LENGTH_MAP] THEN
-`LENGTH (MAP SND stl) >= LENGTH x` by FULL_SIMP_TAC (arith_ss) [LENGTH_APPEND] THEN
-SRW_TAC [] [] THEN
-`?x.take (LENGTH (REVERSE t ++[h])) (MAP SND stl) = SOME x` by METIS_TAC [take_valid] THEN
-FULL_SIMP_TAC (srw_ss()) []])
+Cases_on `l` THEN SRW_TAC [] [] THEN FULL_SIMP_TAC (srw_ss()) [] 
+THENL[
+      FULL_SIMP_TAC (srw_ss()) [take_def, take10] THEN
+      SRW_TAC [] [] THEN
+      FULL_SIMP_TAC (srw_ss()) [] THEN
+      `LENGTH stl = LENGTH (REVERSE t ++ [h] ++ REVERSE pfx)`
+      by METIS_TAC [LENGTH_MAP] THEN
+      FULL_SIMP_TAC (srw_ss()) [],
 
+      SRW_TAC [] [] THEN FULL_SIMP_TAC (srw_ss()) [] THEN FULL_SIMP_TAC (arith_ss) [] THEN
+      `~((LENGTH (REVERSE t) + 1) = 0)` by DECIDE_TAC THEN
+      `LENGTH (REVERSE t ++ [h]) = (LENGTH (REVERSE t) + 1)` by FULL_SIMP_TAC (arith_ss) [rev_nil, LENGTH, LENGTH_APPEND] THEN
+      `take (LENGTH (REVERSE t) + 1) (REVERSE t ++ [h] ++ REVERSE pfx) = SOME (REVERSE t ++ [h])` by METIS_TAC [takenthm] THEN
+      FULL_SIMP_TAC (srw_ss()) [] THEN
 
+      `LENGTH (REVERSE t ++ [h]) = SUC (LENGTH t)` 
+      by FULL_SIMP_TAC (srw_ss()++ARITH_ss) [LENGTH_REVERSE] THEN
+      METIS_TAC [takenthm, APPEND_ASSOC, option_CASES, SOME_11]]);
 
 
 val validStatesAuggrRule = store_thm ("validStatesAuggrRule", 
-``(auggr g st eof = SOME ag) ==> MEM (item l' (r1,TS eof::r2)) itl
-==> validStates ag ((s,itl)::csl) ==> 
-(l'=startSym ag) /\ (r1=[NTS (startSym g)]) /\ (r2=[])``,
+``(auggr g st eof = SOME ag) ⇒ MEM (item l' (r1,TS eof::r2)) itl
+⇒ validStates ag ((s,itl)::csl) ⇒ 
+(l'=startSym ag) ∧ (r1=[NTS (startSym g)]) ∧ (r2=[])``,
 SRW_TAC [] [] THEN
 `validItl ag [item l' (r1,TS eof::r2)]` by METIS_TAC [validStates_def, validStates_append, rgr_r9eq, validItl_append] THEN
 FULL_SIMP_TAC (srw_ss()) [validItl_def, auggr_def, startSym_def, LET_THM] THEN
-Cases_on `~(NTS st IN nonTerminalsML g) /\ ~(TS eof IN terminalsML g)` THEN
+Cases_on `~(NTS st IN nonTerminalsML g) ∧ ~(TS eof IN terminalsML g)` THEN
 FULL_SIMP_TAC (srw_ss()) [] THEN FULL_SIMP_TAC (srw_ss()) [] THEN
 `ag = G (rule st [NTS (startSym g); TS eof]::rules g) st` by METIS_TAC [] THEN
 FULL_SIMP_TAC (srw_ss()) [rules_def, startSym_def] THENL[
@@ -1670,19 +1718,20 @@ METIS_TAC [APPEND, slemma1_4Tmnls, terminalsEq, APPEND_NIL, APPEND_ASSOC],
 SRW_TAC [] [] THEN
 Cases_on `r1` THEN FULL_SIMP_TAC (srw_ss()) [] THEN
 Cases_on `t` THEN FULL_SIMP_TAC (srw_ss()) [],
-METIS_TAC [APPEND, slemma1_4Tmnls, terminalsEq, APPEND_NIL, APPEND_ASSOC]])
+METIS_TAC [APPEND, slemma1_4Tmnls, terminalsEq, APPEND_NIL, APPEND_ASSOC]]);
 
 val mapFstHd = store_thm ("mapFstHd",
-``!l.~(l=[]) ==> (FST (FST (HD l)) = HD (MAP FST (MAP FST l)))``,
-Induct_on `l` THEN SRW_TAC [] [])
+``∀l.~(l=[]) ⇒ (FST (FST (HD l)) = HD (MAP FST (MAP FST l)))``,
+Induct_on `l` THEN SRW_TAC [] []);
 
 val funcCompNegEq = store_thm ("funcCompNegEq",
-``!l.EVERY ($~ o $~ o isTmnlSym) l ==> EVERY isTmnlSym l``,
-Induct_on `l` THEN SRW_TAC [] [])
+``∀l.EVERY ($~ o $~ o isTmnlSym) l ⇒ EVERY isTmnlSym l``,
+Induct_on `l` THEN SRW_TAC [] []);
 
 val listEndNt = store_thm ("listEndNt",
-``!l l' sfx.(l ++ [NTS N] = l' ++ sfx) ==> EVERY isTmnlSym sfx ==> (sfx=[])``,
-Induct_on `sfx` THEN SRW_TAC [] [] THEN
+``∀l l' sfx.(l ++ [NTS N] = l' ++ sfx) ⇒ EVERY isTmnlSym sfx ⇒ (sfx=[])``,
+
+Induct_on `sfx` THEN SRW_TAC [][] THEN
 `LAST (l ++ [NTS N]) = LAST (l' ++ h::sfx)` by METIS_TAC [] THEN
 `LAST ([NTS N]) = LAST (h::sfx)` by METIS_TAC [last_append, NOT_CONS_NIL, APPEND] THEN
 FULL_SIMP_TAC (srw_ss()) [] THEN
@@ -1693,18 +1742,16 @@ FULL_SIMP_TAC (srw_ss()) [] THEN
 `EVERY isTmnlSym sfx` by METIS_TAC [funcCompNegEq] THEN
 Cases_on `sfx` THEN Cases_on `h` THEN FULL_SIMP_TAC (srw_ss()) [isTmnlSym_def] THEN
 SRW_TAC [] [] THEN
-`(FRONT (TS s'::t) ++ [LAST (TS s'::t)]) = (TS s'::t)` by  METIS_TAC [APPEND_FRONT_LAST, NOT_CONS_NIL] THEN
-`EVERY isTmnlSym  (FRONT (TS s'::t) ++ [NTS N])` by METIS_TAC [EVERY_DEF, EVERY_APPEND, isTmnlSym_def] THEN
-FULL_SIMP_TAC (srw_ss()) [isTmnlSym_def])
-
-
-
+`(FRONT (TS s::t) ++ [LAST (TS s::t)]) = (TS s::t)` by  METIS_TAC [APPEND_FRONT_LAST, NOT_CONS_NIL] THEN
+`EVERY isTmnlSym  (FRONT (TS s::t) ++ [NTS N])` by METIS_TAC [EVERY_DEF, EVERY_APPEND, isTmnlSym_def] THEN
+FULL_SIMP_TAC (srw_ss()) [isTmnlSym_def]);
 
 
 val transImpValidItem = store_thm ("transImpValidItem",
-``!s. (slrmac ag = SOME m) /\ (auggr g st eof = SOME ag) /\
-      (trans ag ((initItems ag (rules ag)), vp) = SOME s) ==>
-      !i. validItem ag vp i ==> MEM i s``,
+``∀s. (slrmac ag = SOME m) ∧ (auggr g st eof = SOME ag) ∧
+      (trans ag ((initItems ag (rules ag)), vp) = SOME s) ⇒
+      ∀i. validItem ag vp i ⇒ MEM i s``,
+
 Induct_on `LENGTH vp` THEN FULL_SIMP_TAC (srw_ss()) [] THEN
 SRW_TAC [] [] 
 THENL[
@@ -1728,13 +1775,13 @@ THENL[
       FULL_SIMP_TAC (srw_ss()) [] THEN 
       Cases_on `moveDot x t` THEN
       FULL_SIMP_TAC (srw_ss()) [] THEN
-      `((pfx'=pfx) /\ (q=[t])) \/
-       (?q1 q2.(q=q1++q2) /\ (pfx=pfx'++q1) /\ ([t]=q2)) \/
-       (?t1 t2.([t]=t1++t2) /\ (pfx'=pfx++t1) /\ (q=t2))` by METIS_TAC [twoListAppEq] THEN
+      `((pfx'=pfx) ∧ (q=[t])) ∨
+       (∃q1 q2.(q=q1++q2) ∧ (pfx=pfx'++q1) ∧ ([t]=q2)) ∨
+       (∃t1 t2.([t]=t1++t2) ∧ (pfx'=pfx++t1) ∧ (q=t2))` by METIS_TAC [twoListAppEq] THEN
       SRW_TAC [] [] 
       THENL[
-	    `?s.(trans ag (initItems ag (rules ag),pfx) = SOME s) 
-                /\ MEM (item s' ([],[t]++r)) s` 
+	    `∃s.(trans ag (initItems ag (rules ag),pfx) = SOME s) 
+                ∧ MEM (item n ([],[t]++r)) s` 
 		by METIS_TAC [lemma, RTC_NRC] THEN
 	    `x=s` by METIS_TAC [transOutEq] THEN
 	    SRW_TAC [] [] THEN
@@ -1743,11 +1790,11 @@ THENL[
 	    FULL_SIMP_TAC (srw_ss()) [md_append, moveDot_def] THEN
 	    METIS_TAC [iclosure_mem, MEM, MEM_APPEND, rgr_r9eq],
 
-	    `?s.(trans ag (initItems ag (rules ag),pfx') = SOME s) 
-               /\ MEM (item s' ([],q1++[t]++r)) s` 
+	    `∃s.(trans ag (initItems ag (rules ag),pfx') = SOME s) 
+               ∧ MEM (item n ([],q1++[t]++r)) s` 
 		by METIS_TAC [lemma, RTC_NRC] THEN
-	    `?st.(trans ag (s,q1) = SOME st) 
-                  /\ MEM (item s' ([]++q1,[t]++r)) st` 
+	    `∃st.(trans ag (s,q1) = SOME st) 
+                  ∧ MEM (item n ([]++q1,[t]++r)) st` 
 		by METIS_TAC [transExists, APPEND_ASSOC] THEN
 	    FULL_SIMP_TAC (srw_ss()) []THEN
 	    `trans ag (initItems ag (rules ag),pfx'++q1) = SOME st'` 
@@ -1761,8 +1808,8 @@ THENL[
 
 
 	    SRW_TAC [] [] THEN
-	    `?s.(trans ag (initItems ag (rules ag),pfx++t1) = SOME s) 
-               /\ MEM (item s' ([],q++r)) s` 
+	    `∃s.(trans ag (initItems ag (rules ag),pfx++t1) = SOME s) 
+               ∧ MEM (item n ([],q++r)) s` 
 		by METIS_TAC [lemma, RTC_NRC] THEN
 	    Cases_on `t1` THEN Cases_on `q` THEN SRW_TAC [] [] THEN
 	    FULL_SIMP_TAC (srw_ss()) [] THEN
@@ -1781,6 +1828,6 @@ THENL[
 		  FULL_SIMP_TAC (srw_ss()) [] THEN
 		  SRW_TAC [] [] THEN
 		  METIS_TAC []
-		  ]]])
+		  ]]]);
 
 val _ = export_theory()
